txn-data-consistency/EP+_Invariants_Proof.thy
@@ -1,7 +1,7 @@
-section \<open>Eiger Port Plus Protocol Satisfying CCv (Causal+) - Proofs and lemmas\<close>
+section \<open>Eiger Port Plus Protocol (not sorted) - Proofs and lemmas\<close>
 
-theory "EP+_TCCv_Proof"
-  imports "EP+_Sorted"
+theory "EP+_Invariants_Proof"
+  imports "EP+"
 begin
 
 subsection \<open>wtxns lemmas\<close>
@@ -380,9 +380,6 @@ lemma fold_pending_wtxns_fun_upd:
    pending_wtxns_ts (m (t := b))"
   by (simp add: fun_upd_def)
 
-lemma not_less_eq: "\<not>((a :: nat) < b) \<Longrightarrow> a \<noteq> b \<Longrightarrow> a > b" by simp
-
-
 subsection \<open>Invariants about initializations and finity of kvs and its versions\<close>
 
 definition T0_in_CO where
@@ -391,11 +388,11 @@ definition T0_in_CO where
 lemmas T0_in_COI = T0_in_CO_def[THEN iffD2, rule_format]
 lemmas T0_in_COE[elim] = T0_in_CO_def[THEN iffD1, elim_format, rule_format]
 
-lemma reach_t0_in_co [simp, dest]: "reach tps_s s \<Longrightarrow> T0_in_CO s k"
+lemma reach_t0_in_co [simp, dest]: "reach tps s \<Longrightarrow> T0_in_CO s k"
 proof(induction s rule: reach.induct)
   case (reach_init s)
   then show ?case
-    by (auto simp add: T0_in_CO_def tps_s_defs)
+    by (auto simp add: T0_in_CO_def tps_defs)
 next
   case (reach_trans s e s')
   then show ?case
@@ -412,11 +409,11 @@ definition Kvs_Not_Emp where
 lemmas Kvs_Not_EmpI = Kvs_Not_Emp_def[THEN iffD2, rule_format]
 lemmas Kvs_Not_EmpE[elim] = Kvs_Not_Emp_def[THEN iffD1, elim_format, rule_format]
 
-lemma reach_kvs_not_emp [simp]: "reach tps_s s \<Longrightarrow> Kvs_Not_Emp s"
+lemma reach_kvs_not_emp [simp]: "reach tps s \<Longrightarrow> Kvs_Not_Emp s"
 proof(induction s rule: reach.induct)
   case (reach_init s)
   then show ?case
-    apply (auto simp add: Kvs_Not_Emp_def tps_s_defs)
+    apply (auto simp add: Kvs_Not_Emp_def tps_defs)
     by (metis fun_upd_apply ver_state.distinct(3))
 next
   case (reach_trans s e s')
@@ -439,15 +436,7 @@ next
   qed (auto simp add: Kvs_Not_Emp_def tps_trans_defs)
 qed
 
-definition KvsOfS_Not_Emp where
-  "KvsOfS_Not_Emp s \<longleftrightarrow> (\<forall>k. kvs_of_s s k \<noteq> [])"
-
-lemmas KvsOfS_Not_EmpI = KvsOfS_Not_Emp_def[THEN iffD2, rule_format]
-lemmas KvsOfS_Not_EmpE[elim] = KvsOfS_Not_Emp_def[THEN iffD1, elim_format, rule_format]
-
-lemma reach_kvs_of_s_not_emp [simp]: "reach tps_s s \<Longrightarrow> KvsOfS_Not_Emp s"
-  apply (auto simp add: KvsOfS_Not_Emp_def T0_in_CO_def kvs_of_s_defs)
-  by (smt (verit) T0_in_CO_def empty_iff empty_set reach_t0_in_co)
+(****** KvsOfS_Not_Emp *****)
 
 definition Dom_Kv_map_Not_Emp where
   "Dom_Kv_map_Not_Emp s cl \<longleftrightarrow> 
@@ -457,10 +446,10 @@ definition Dom_Kv_map_Not_Emp where
 lemmas Dom_Kv_map_Not_EmpI = Dom_Kv_map_Not_Emp_def[THEN iffD2, rule_format]
 lemmas Dom_Kv_map_Not_EmpE[elim] = Dom_Kv_map_Not_Emp_def[THEN iffD1, elim_format, rule_format]
 
-lemma reach_dom_kv_map_not_emp [simp]: "reach tps_s s \<Longrightarrow> Dom_Kv_map_Not_Emp s cl"
+lemma reach_dom_kv_map_not_emp [simp]: "reach tps s \<Longrightarrow> Dom_Kv_map_Not_Emp s cl"
 proof(induction s rule: reach.induct)
   case (reach_init s)
-  then show ?case by (auto simp add: Dom_Kv_map_Not_Emp_def tps_s_defs)
+  then show ?case by (auto simp add: Dom_Kv_map_Not_Emp_def tps_defs)
 next
   case (reach_trans s e s')
   then show ?case
@@ -473,11 +462,11 @@ definition Init_Ver_Inv where
 lemmas Init_Ver_InvI = Init_Ver_Inv_def[THEN iffD2, rule_format]
 lemmas Init_Ver_InvE[elim] = Init_Ver_Inv_def[THEN iffD1, elim_format, rule_format]
 
-lemma reach_init_ver_inv [simp, intro]: "reach tps_s s \<Longrightarrow> Init_Ver_Inv s k"
+lemma reach_init_ver_inv [simp, intro]: "reach tps s \<Longrightarrow> Init_Ver_Inv s k"
 proof(induction s rule: reach.induct)
   case (reach_init s)
   then show ?case
-    by (auto simp add: Init_Ver_Inv_def tps_s_defs)
+    by (auto simp add: Init_Ver_Inv_def tps_defs)
 next
   case (reach_trans s e s')
   then show ?case
@@ -494,10 +483,10 @@ definition Finite_Wtxns_Dom where
 lemmas Finite_Wtxns_DomI = Finite_Wtxns_Dom_def[THEN iffD2, rule_format]
 lemmas Finite_Wtxns_DomE[elim] = Finite_Wtxns_Dom_def[THEN iffD1, elim_format, rule_format]
 
-lemma reach_finite_wtxns_dom [simp]: "reach tps_s s \<Longrightarrow> Finite_Wtxns_Dom s k"
+lemma reach_finite_wtxns_dom [simp]: "reach tps s \<Longrightarrow> Finite_Wtxns_Dom s k"
 proof(induction s rule: reach.induct)
   case (reach_init s)
-  then show ?case apply (auto simp add: Finite_Wtxns_Dom_def tps_s_defs)
+  then show ?case apply (auto simp add: Finite_Wtxns_Dom_def tps_defs)
     by (metis finite.emptyI wtxns_dom_eq_empty_conv)
 next
   case (reach_trans s e s')
@@ -516,10 +505,10 @@ definition Finite_Wtxns_rsran where
 lemmas Finite_Wtxns_rsranI = Finite_Wtxns_rsran_def[THEN iffD2, rule_format]
 lemmas Finite_Wtxns_rsranE[elim] = Finite_Wtxns_rsran_def[THEN iffD1, elim_format, rule_format]
 
-lemma reach_finite_wtxns_rsran [simp]: "reach tps_s s \<Longrightarrow> Finite_Wtxns_rsran s k"
+lemma reach_finite_wtxns_rsran [simp]: "reach tps s \<Longrightarrow> Finite_Wtxns_rsran s k"
 proof(induction s rule: reach.induct)
   case (reach_init s)
-  then show ?case by (auto simp add: Finite_Wtxns_rsran_def tps_s_defs)
+  then show ?case by (auto simp add: Finite_Wtxns_rsran_def tps_defs)
 next
   case (reach_trans s e s')
   then show ?case
@@ -537,11 +526,11 @@ definition Finite_Pend_Inv where
 lemmas Finite_Pend_InvI = Finite_Pend_Inv_def[THEN iffD2, rule_format]
 lemmas Finite_Pend_InvE[elim] = Finite_Pend_Inv_def[THEN iffD1, elim_format, rule_format]
 
-lemma reach_finitepending [simp]: "reach tps_s s \<Longrightarrow> Finite_Pend_Inv s k"
+lemma reach_finitepending [simp]: "reach tps s \<Longrightarrow> Finite_Pend_Inv s k"
 proof(induction s rule: reach.induct)
   case (reach_init s)
   then show ?case
-  by (auto simp add: Finite_Pend_Inv_def tps_s_defs pending_wtxns_ts_def)
+  by (auto simp add: Finite_Pend_Inv_def tps_defs pending_wtxns_ts_def)
 next
   case (reach_trans s e s')
   then show ?case 
@@ -568,11 +557,11 @@ definition Finite_Dom_Kv_map where
 lemmas Finite_Dom_Kv_mapI = Finite_Dom_Kv_map_def[THEN iffD2, rule_format]
 lemmas Finite_Dom_Kv_mapE[elim] = Finite_Dom_Kv_map_def[THEN iffD1, elim_format, rule_format]
          
-lemma reach_finite_dom_kv_map [simp]: "reach tps_s s \<Longrightarrow> Finite_Dom_Kv_map s cl"
+lemma reach_finite_dom_kv_map [simp]: "reach tps s \<Longrightarrow> Finite_Dom_Kv_map s cl"
 proof(induction s rule: reach.induct)
   case (reach_init s)
   then show ?case
-  by (auto simp add: Finite_Dom_Kv_map_def tps_s_defs)
+  by (auto simp add: Finite_Dom_Kv_map_def tps_defs)
 next
   case (reach_trans s e s')
   then show ?case
@@ -587,11 +576,11 @@ definition Finite_Dom_Kv_map_rd where
 lemmas Finite_Dom_Kv_map_rdI = Finite_Dom_Kv_map_rd_def[THEN iffD2, rule_format]
 lemmas Finite_Dom_Kv_map_rdE[elim] = Finite_Dom_Kv_map_rd_def[THEN iffD1, elim_format, rule_format]
          
-lemma reach_finite_dom_kv_map_rd [simp]: "reach tps_s s \<Longrightarrow> Finite_Dom_Kv_map_rd s cl"
+lemma reach_finite_dom_kv_map_rd [simp]: "reach tps s \<Longrightarrow> Finite_Dom_Kv_map_rd s cl"
 proof(induction s rule: reach.induct)
   case (reach_init s)
   then show ?case
-  by (auto simp add: Finite_Dom_Kv_map_rd_def tps_s_defs)
+  by (auto simp add: Finite_Dom_Kv_map_rd_def tps_defs)
 next
   case (reach_trans s e s')
   then show ?case
@@ -605,11 +594,11 @@ definition Finite_Keys where
 lemmas Finite_KeysI = Finite_Keys_def[THEN iffD2, rule_format]
 lemmas Finite_KeysE[elim] = Finite_Keys_def[THEN iffD1, elim_format, rule_format]
          
-lemma reach_finite_keys [simp]: "reach tps_s s \<Longrightarrow> Finite_Keys s cl"
+lemma reach_finite_keys [simp]: "reach tps s \<Longrightarrow> Finite_Keys s cl"
 proof(induction s rule: reach.induct)
   case (reach_init s)
   then show ?case
-  by (auto simp add: Finite_Keys_def tps_s_defs)
+  by (auto simp add: Finite_Keys_def tps_defs)
 next
   case (reach_trans s e s')
   then show ?case
@@ -622,11 +611,11 @@ definition Finite_Lst_map_Ran where
 lemmas Finite_Lst_map_RanI = Finite_Lst_map_Ran_def[THEN iffD2, rule_format]
 lemmas Finite_Lst_map_RanE[elim] = Finite_Lst_map_Ran_def[THEN iffD1, elim_format, rule_format]
          
-lemma reach_finite_lst_map_ran [simp]: "reach tps_s s \<Longrightarrow> Finite_Lst_map_Ran s cl"
+lemma reach_finite_lst_map_ran [simp]: "reach tps s \<Longrightarrow> Finite_Lst_map_Ran s cl"
 proof(induction s rule: reach.induct)
   case (reach_init s)
   then show ?case
-  by (auto simp add: Finite_Lst_map_Ran_def tps_s_defs)
+  by (auto simp add: Finite_Lst_map_Ran_def tps_defs)
 next
   case (reach_trans s e s')
   then show ?case
@@ -643,7 +632,7 @@ next
 qed
 
 lemma finite_get_ts:
-  "reach tps_s s \<Longrightarrow>
+  "reach tps s \<Longrightarrow>
    cl_state (cls s cl) \<in> {WtxnPrep kv_map, WtxnCommit cts kv_map} \<Longrightarrow>
    finite {get_ts (svr_state (svrs s k) (get_wtxn s cl)) |k. k \<in> dom kv_map}"
   using Finite_Dom_Kv_map_def[of s cl] dom_def by auto
@@ -760,11 +749,11 @@ definition FTid_Wtxn_Inv where
 lemmas FTid_Wtxn_InvI = FTid_Wtxn_Inv_def[THEN iffD2, rule_format]
 lemmas FTid_Wtxn_InvE[elim] = FTid_Wtxn_Inv_def[THEN iffD1, elim_format, rule_format]
 
-lemma reach_ftid_wtxn_inv [simp, dest]: "reach tps_s s \<Longrightarrow> FTid_Wtxn_Inv s cl"
+lemma reach_ftid_wtxn_inv [simp, dest]: "reach tps s \<Longrightarrow> FTid_Wtxn_Inv s cl"
 proof(induction s rule: reach.induct)
   case (reach_init s)
   then show ?case
-  by (auto simp add: FTid_Wtxn_Inv_def tps_s_defs)
+  by (auto simp add: FTid_Wtxn_Inv_def tps_defs)
 next
   case (reach_trans s e s')
   then show ?case 
@@ -786,11 +775,11 @@ definition Cl_Rtxn_Inv where
 lemmas Cl_Rtxn_InvI = Cl_Rtxn_Inv_def[THEN iffD2, rule_format]
 lemmas Cl_Rtxn_InvE[elim] = Cl_Rtxn_Inv_def[THEN iffD1, elim_format, rule_format]
 
-lemma reach_cl_rtxn_inv [simp, dest]: "reach tps_s s \<Longrightarrow> Cl_Rtxn_Inv s cl"
+lemma reach_cl_rtxn_inv [simp, dest]: "reach tps s \<Longrightarrow> Cl_Rtxn_Inv s cl"
 proof(induction s rule: reach.induct)
   case (reach_init s)
   then show ?case
-  by (auto simp add: Cl_Rtxn_Inv_def tps_s_defs)
+  by (auto simp add: Cl_Rtxn_Inv_def tps_defs)
 next
   case (reach_trans s e s')
   then show ?case 
@@ -810,18 +799,18 @@ next
 qed
 
 definition Cl_Wtxn_Idle_Svr where
-  "Cl_Wtxn_Idle_Svr s \<longleftrightarrow>
-    (\<forall>cl k cts kv_map. cl_state (cls s cl) \<in> {WtxnPrep kv_map, WtxnCommit cts kv_map}
+  "Cl_Wtxn_Idle_Svr s cl k \<longleftrightarrow>
+    (\<forall>cts kv_map. cl_state (cls s cl) \<in> {WtxnPrep kv_map, WtxnCommit cts kv_map}
         \<and> kv_map k = None \<longrightarrow> svr_state (svrs s k) (get_wtxn s cl) = No_Ver)"
 
 lemmas Cl_Wtxn_Idle_SvrI = Cl_Wtxn_Idle_Svr_def[THEN iffD2, rule_format]
 lemmas Cl_Wtxn_Idle_SvrE[elim] = Cl_Wtxn_Idle_Svr_def[THEN iffD1, elim_format, rule_format]
 
-lemma reach_cl_wtxn_idle_svr [simp]: "reach tps_s s \<Longrightarrow> Cl_Wtxn_Idle_Svr s"
+lemma reach_cl_wtxn_idle_svr [simp]: "reach tps s \<Longrightarrow> Cl_Wtxn_Idle_Svr s cl k"
 proof(induction s rule: reach.induct)
   case (reach_init s)
   then show ?case
-  by (auto simp add: Cl_Wtxn_Idle_Svr_def tps_s_defs)
+  by (auto simp add: Cl_Wtxn_Idle_Svr_def tps_defs)
 next
   case (reach_trans s e s')
   then show ?case 
@@ -848,11 +837,11 @@ definition Cl_Prep_Inv where
 lemmas Cl_Prep_InvI = Cl_Prep_Inv_def[THEN iffD2, rule_format]
 lemmas Cl_Prep_InvE[elim] = Cl_Prep_Inv_def[THEN iffD1, elim_format, rule_format]
 
-lemma reach_cl_prep_inv [simp]: "reach tps_s s \<Longrightarrow> Cl_Prep_Inv s"
+lemma reach_cl_prep_inv [simp]: "reach tps s \<Longrightarrow> Cl_Prep_Inv s"
 proof(induction s rule: reach.induct)
   case (reach_init s)
   then show ?case
-  by (auto simp add: Cl_Prep_Inv_def tps_s_defs)
+  by (auto simp add: Cl_Prep_Inv_def tps_defs)
 next
   case (reach_trans s e s')
   then show ?case 
@@ -883,11 +872,11 @@ definition Cl_Commit_Inv where
 lemmas Cl_Commit_InvI = Cl_Commit_Inv_def[THEN iffD2, rule_format]
 lemmas Cl_Commit_InvE[elim] = Cl_Commit_Inv_def[THEN iffD1, elim_format, rule_format]
 
-lemma reach_cl_commit_inv [simp]: "reach tps_s s \<Longrightarrow> Cl_Commit_Inv s cl k"
+lemma reach_cl_commit_inv [simp]: "reach tps s \<Longrightarrow> Cl_Commit_Inv s cl k"
 proof(induction s rule: reach.induct)
   case (reach_init s)
   then show ?case
-  by (auto simp add: Cl_Commit_Inv_def tps_s_defs)
+  by (auto simp add: Cl_Commit_Inv_def tps_defs)
 next
   case (reach_trans s e s')
   then show ?case 
@@ -920,11 +909,11 @@ definition Prep_is_Curr_wt where
 lemmas Prep_is_Curr_wtI = Prep_is_Curr_wt_def[THEN iffD2, rule_format]
 lemmas Prep_is_Curr_wtE[elim] = Prep_is_Curr_wt_def[THEN iffD1, elim_format, rule_format]
 
-lemma reach_prep_is_curr_wt[simp]: "reach tps_s s \<Longrightarrow> Prep_is_Curr_wt s k"
+lemma reach_prep_is_curr_wt[simp]: "reach tps s \<Longrightarrow> Prep_is_Curr_wt s k"
 proof(induction s rule: reach.induct)
   case (reach_init s)
   then show ?case
-    by (auto simp add: Prep_is_Curr_wt_def tps_s_defs split: if_split_asm)
+    by (auto simp add: Prep_is_Curr_wt_def tps_defs split: if_split_asm)
 next
   case (reach_trans s e s')
   then show ?case
@@ -936,10 +925,13 @@ next
   next
     case (WDone x1 x2 x3 x4 x5)
     then show ?case apply (auto simp add: Prep_is_Curr_wt_def tps_trans_defs)
-    apply (cases "x2 k")
-       apply (smt (z3) Cl_Wtxn_Idle_Svr_def get_cl_w.simps(2) get_sn_w.cases get_sn_w.simps(2)
+    apply (cases "x2 k") 
+       apply (smt (verit) Cl_Wtxn_Idle_Svr_def get_cl_w.simps(2) get_sn_w.cases get_sn_w.simps(2)
+          insert_iff is_prepared.simps(2) reach_cl_wtxn_idle_svr)
+       (*changed from:
+         apply (smt (z3) Cl_Wtxn_Idle_Svr_def get_cl_w.simps(2) get_sn_w.cases get_sn_w.simps(2)
           insert_commute insert_compr insert_iff is_prepared.elims(1) reach_cl_wtxn_idle_svr
-          ver_state.distinct(1))
+          ver_state.distinct(1)*)
       by (smt domI get_cl_w.simps(2) get_sn_w.cases get_sn_w.simps(2) is_prepared.simps(3)
           mem_Collect_eq option.discI)
   next
@@ -962,10 +954,10 @@ definition Svr_Prep_Inv where
 lemmas Svr_Prep_InvI = Svr_Prep_Inv_def[THEN iffD2, rule_format]
 lemmas Svr_Prep_InvE[elim] = Svr_Prep_Inv_def[THEN iffD1, elim_format, rule_format]
 
-lemma reach_svr_prep_inv [simp]: "reach tps_s s \<Longrightarrow> Svr_Prep_Inv s"
+lemma reach_svr_prep_inv [simp]: "reach tps s \<Longrightarrow> Svr_Prep_Inv s"
 proof(induction s rule: reach.induct)
   case (reach_init s)
-  then show ?case by (auto simp add: Svr_Prep_Inv_def tps_s_defs split: if_split_asm)
+  then show ?case by (auto simp add: Svr_Prep_Inv_def tps_defs split: if_split_asm)
 next
   case (reach_trans s e s')
   then show ?case 
@@ -1014,10 +1006,10 @@ definition Svr_Commit_Inv where
 lemmas Svr_Commit_InvI = Svr_Commit_Inv_def[THEN iffD2, rule_format]
 lemmas Svr_Commit_InvE[elim] = Svr_Commit_Inv_def[THEN iffD1, elim_format, rule_format]
 
-lemma reach_svr_commit_inv [simp]: "reach tps_s s \<Longrightarrow> Svr_Commit_Inv s"
+lemma reach_svr_commit_inv [simp]: "reach tps s \<Longrightarrow> Svr_Commit_Inv s"
 proof(induction s rule: reach.induct)
   case (reach_init s)
-  then show ?case by (auto simp add: Svr_Commit_Inv_def tps_s_defs)
+  then show ?case by (auto simp add: Svr_Commit_Inv_def tps_defs)
 next
   case (reach_trans s e s')
   then show ?case 
@@ -1067,10 +1059,10 @@ definition CFTid_Rtxn_Inv where
 lemmas CFTid_Rtxn_InvI = CFTid_Rtxn_Inv_def[THEN iffD2, rule_format]
 lemmas CFTid_Rtxn_InvE[elim] = CFTid_Rtxn_Inv_def[THEN iffD1, elim_format, rule_format]
 
-lemma reach_cftid_rtxn_inv [simp]: "reach tps_s s \<Longrightarrow> CFTid_Rtxn_Inv s cl"
+lemma reach_cftid_rtxn_inv [simp]: "reach tps s \<Longrightarrow> CFTid_Rtxn_Inv s cl"
 proof(induction s rule: reach.induct)
   case (reach_init s)
-  then show ?case by (auto simp add: CFTid_Rtxn_Inv_def tps_s_defs)
+  then show ?case by (auto simp add: CFTid_Rtxn_Inv_def tps_defs)
 next
   case (reach_trans s e s')
   then show ?case by (induction e) (auto simp add: CFTid_Rtxn_Inv_def tps_trans_defs)
@@ -1117,10 +1109,10 @@ definition CTid_Cts where
 lemmas CTid_CtsI = CTid_Cts_def[THEN iffD2, rule_format]
 lemmas CTid_CtsE[elim] = CTid_Cts_def[THEN iffD1, elim_format, rule_format]
 
-lemma reach_ctid_cts_inv [simp]: "reach tps_s s \<Longrightarrow> CTid_Cts s cl"
+lemma reach_ctid_cts_inv [simp]: "reach tps s \<Longrightarrow> CTid_Cts s cl"
 proof(induction s rule: reach.induct)
   case (reach_init s)
-  then show ?case by (auto simp add: CTid_Cts_def tps_s_defs)
+  then show ?case by (auto simp add: CTid_Cts_def tps_defs)
 next
   case (reach_trans s e s')
   then show ?case
@@ -1156,10 +1148,10 @@ definition FTid_notin_rs where
 lemmas FTid_notin_rsI = FTid_notin_rs_def[THEN iffD2, rule_format]
 lemmas FTid_notin_rsE[elim] = FTid_notin_rs_def[THEN iffD1, elim_format, rule_format]
 
-lemma reach_ftid_notin_rs [simp, dest]: "reach tps_s s \<Longrightarrow> FTid_notin_rs s cl"
+lemma reach_ftid_notin_rs [simp, dest]: "reach tps s \<Longrightarrow> FTid_notin_rs s cl"
 proof(induction s rule: reach.induct)
   case (reach_init s)
-  then show ?case by (auto simp add: FTid_notin_rs_def tps_s_defs split: if_split_asm)
+  then show ?case by (auto simp add: FTid_notin_rs_def tps_defs split: if_split_asm)
 next
   case (reach_trans s e s')
   then show ?case 
@@ -1195,11 +1187,11 @@ definition FTid_not_wr where
 lemmas FTid_not_wrI = FTid_not_wr_def[THEN iffD2, rule_format]
 lemmas FTid_not_wrE[elim] = FTid_not_wr_def[THEN iffD1, elim_format, rule_format]
 
-lemma reach_ftid_not_wr [simp]: "reach tps_s s \<Longrightarrow> FTid_not_wr s cl"
+lemma reach_ftid_not_wr [simp]: "reach tps s \<Longrightarrow> FTid_not_wr s cl"
 proof(induction s rule: reach.induct)
   case (reach_init s)
   then show ?case
-  by (auto simp add: FTid_not_wr_def tps_s_defs)
+  by (auto simp add: FTid_not_wr_def tps_defs)
 next
   case (reach_trans s e s')
   then show ?case 
@@ -1234,11 +1226,11 @@ definition Fresh_wr_notin_Wts_dom where
 lemmas Fresh_wr_notin_Wts_domI = Fresh_wr_notin_Wts_dom_def[THEN iffD2, rule_format]
 lemmas Fresh_wr_notin_Wts_domE[elim] = Fresh_wr_notin_Wts_dom_def[THEN iffD1, elim_format, rule_format]
 
-lemma reach_fresh_wr_notin_wtxns_dom [simp]: "reach tps_s s \<Longrightarrow> Fresh_wr_notin_Wts_dom s cl"
+lemma reach_fresh_wr_notin_wtxns_dom [simp]: "reach tps s \<Longrightarrow> Fresh_wr_notin_Wts_dom s cl"
 proof(induction s rule: reach.induct)
   case (reach_init s)
   then show ?case
-  by (auto simp add: Fresh_wr_notin_Wts_dom_def tps_s_defs)
+  by (auto simp add: Fresh_wr_notin_Wts_dom_def tps_defs)
 next
   case (reach_trans s e s')
   then show ?case 
@@ -1263,10 +1255,10 @@ definition Fresh_wr_notin_rs where
 lemmas Fresh_wr_notin_rsI = Fresh_wr_notin_rs_def[THEN iffD2, rule_format]
 lemmas Fresh_wr_notin_rsE[elim] = Fresh_wr_notin_rs_def[THEN iffD1, elim_format, rule_format]
 
-lemma reach_fresh_wr_notin_rs [simp]: "reach tps_s s \<Longrightarrow> Fresh_wr_notin_rs s cl"
+lemma reach_fresh_wr_notin_rs [simp]: "reach tps s \<Longrightarrow> Fresh_wr_notin_rs s cl"
 proof(induction s rule: reach.induct)
   case (reach_init s)
-  then show ?case by (auto simp add: Fresh_wr_notin_rs_def tps_s_defs split: if_split_asm)
+  then show ?case by (auto simp add: Fresh_wr_notin_rs_def tps_defs split: if_split_asm)
 next
   case (reach_trans s e s')
   then show ?case 
@@ -1297,11 +1289,11 @@ definition PTid_Inv where
 lemmas PTid_InvI = PTid_Inv_def[THEN iffD2, rule_format]
 lemmas PTid_InvE[elim] = PTid_Inv_def[THEN iffD1, elim_format, rule_format]
 
-lemma reach_ptid_inv [simp]: "reach tps_s s \<Longrightarrow> PTid_Inv s cl"
+lemma reach_ptid_inv [simp]: "reach tps s \<Longrightarrow> PTid_Inv s cl"
 proof(induction s rule: reach.induct)
   case (reach_init s)
   then show ?case
-  by (auto simp add: PTid_Inv_def tps_s_defs)
+  by (auto simp add: PTid_Inv_def tps_defs)
 next
   case (reach_trans s e s')
   then show ?case 
@@ -1348,10 +1340,10 @@ definition Rtxn_Wtxn_No_Ver where
 lemmas Rtxn_Wtxn_No_VerI = Rtxn_Wtxn_No_Ver_def[THEN iffD2, rule_format]
 lemmas Rtxn_Wtxn_No_VerE[elim] = Rtxn_Wtxn_No_Ver_def[THEN iffD1, elim_format, rule_format]
 
-lemma reach_rtxn_wtxn_no_ver [simp]: "reach tps_s s \<Longrightarrow> Rtxn_Wtxn_No_Ver s cl"
+lemma reach_rtxn_wtxn_no_ver [simp]: "reach tps s \<Longrightarrow> Rtxn_Wtxn_No_Ver s cl"
 proof(induction s rule: reach.induct)
   case (reach_init s)
-  then show ?case by (auto simp add: Rtxn_Wtxn_No_Ver_def tps_s_defs)
+  then show ?case by (auto simp add: Rtxn_Wtxn_No_Ver_def tps_defs)
 next
   case (reach_trans s e s')
   then show ?case 
@@ -1378,10 +1370,10 @@ definition Wtxn_Rtxn_None where
 lemmas Wtxn_Rtxn_NoneI = Wtxn_Rtxn_None_def[THEN iffD2, rule_format]
 lemmas Wtxn_Rtxn_NoneE[elim] = Wtxn_Rtxn_None_def[THEN iffD1, elim_format, rule_format]
 
-lemma reach_wtxn_rtxn_none [simp]: "reach tps_s s \<Longrightarrow> Wtxn_Rtxn_None s k"
+lemma reach_wtxn_rtxn_none [simp]: "reach tps s \<Longrightarrow> Wtxn_Rtxn_None s k"
 proof(induction s rule: reach.induct)
   case (reach_init s)
-  then show ?case by (auto simp add: Wtxn_Rtxn_None_def tps_s_defs)
+  then show ?case by (auto simp add: Wtxn_Rtxn_None_def tps_defs)
 next
   case (reach_trans s e s')
   then show ?case using Cl_Rtxn_Inv_def[of s]
@@ -1407,11 +1399,11 @@ definition Wtxn_Cts_T0 where
 lemmas Wtxn_Cts_T0I = Wtxn_Cts_T0_def[THEN iffD2, rule_format]
 lemmas Wtxn_Cts_T0E[elim] = Wtxn_Cts_T0_def[THEN iffD1, elim_format, rule_format]
 
-lemma reach_wtxn_cts_t0 [simp, dest]: "reach tps_s s \<Longrightarrow> Wtxn_Cts_T0 s"
+lemma reach_wtxn_cts_t0 [simp, dest]: "reach tps s \<Longrightarrow> Wtxn_Cts_T0 s"
 proof(induction s rule: reach.induct)
   case (reach_init s)
   then show ?case
-    by (auto simp add: Wtxn_Cts_T0_def tps_s_defs)
+    by (auto simp add: Wtxn_Cts_T0_def tps_defs)
 next
   case (reach_trans s e s')
   then show ?case
@@ -1427,11 +1419,11 @@ definition Wtxn_Cts_Tn_None where
 lemmas Wtxn_Cts_Tn_NoneI = Wtxn_Cts_Tn_None_def[THEN iffD2, rule_format]
 lemmas Wtxn_Cts_Tn_NoneE[elim] = Wtxn_Cts_Tn_None_def[THEN iffD1, elim_format, rule_format]
 
-lemma reach_wtxn_cts_tn_none [simp, intro]: "reach tps_s s \<Longrightarrow> Wtxn_Cts_Tn_None s"
+lemma reach_wtxn_cts_tn_none [simp, intro]: "reach tps s \<Longrightarrow> Wtxn_Cts_Tn_None s"
 proof(induction s rule: reach.induct)
   case (reach_init s)
   then show ?case
-    by (auto simp add: Wtxn_Cts_Tn_None_def tps_s_defs)
+    by (auto simp add: Wtxn_Cts_Tn_None_def tps_defs)
 next
   case (reach_trans s e s')
   then show ?case
@@ -1449,7 +1441,7 @@ definition Wtxn_Cts_None where
 lemmas Wtxn_Cts_NoneI = Wtxn_Cts_None_def[THEN iffD2, rule_format]
 lemmas Wtxn_Cts_NoneE[elim] = Wtxn_Cts_None_def[THEN iffD1, elim_format, rule_format]
 
-lemma reach_wtxn_cts_none [simp, intro]: "reach tps_s s \<Longrightarrow> Wtxn_Cts_None s"
+lemma reach_wtxn_cts_none [simp, intro]: "reach tps s \<Longrightarrow> Wtxn_Cts_None s"
   apply (simp add: Wtxn_Cts_None_def)
   apply rule+ subgoal for cts kv_map cclk keys t apply (cases t)
     apply metis using Wtxn_Cts_Tn_None_def[of s]
@@ -1462,11 +1454,11 @@ definition WtxnCommit_Wtxn_Cts where
 lemmas WtxnCommit_Wtxn_CtsI = WtxnCommit_Wtxn_Cts_def[THEN iffD2, rule_format]
 lemmas WtxnCommit_Wtxn_CtsE[elim] = WtxnCommit_Wtxn_Cts_def[THEN iffD1, elim_format, rule_format]
 
-lemma reach_wtxncommit_wtxn_cts [simp, intro]: "reach tps_s s \<Longrightarrow> WtxnCommit_Wtxn_Cts s cl"
+lemma reach_wtxncommit_wtxn_cts [simp, intro]: "reach tps s \<Longrightarrow> WtxnCommit_Wtxn_Cts s cl"
 proof(induction s rule: reach.induct)
   case (reach_init s)
   then show ?case
-    by (auto simp add: WtxnCommit_Wtxn_Cts_def tps_s_defs)
+    by (auto simp add: WtxnCommit_Wtxn_Cts_def tps_defs)
 next
   case (reach_trans s e s')
   then show ?case
@@ -1482,10 +1474,10 @@ definition Wtxn_State_Cts where
 lemmas Wtxn_State_CtsI = Wtxn_State_Cts_def[THEN iffD2, rule_format]
 lemmas Wtxn_State_CtsE[elim] = Wtxn_State_Cts_def[THEN iffD1, elim_format, rule_format]
 
-lemma reach_svr_state_cts [simp]: "reach tps_s s \<Longrightarrow> Wtxn_State_Cts s k"
+lemma reach_svr_state_cts [simp]: "reach tps s \<Longrightarrow> Wtxn_State_Cts s k"
 proof(induction s rule: reach.induct)
   case (reach_init s)
-  then show ?case by (auto simp add: Wtxn_State_Cts_def tps_s_defs split: if_split_asm)
+  then show ?case by (auto simp add: Wtxn_State_Cts_def tps_defs split: if_split_asm)
 next
   case (reach_trans s e s')
   then show ?case
@@ -1530,10 +1522,10 @@ definition Cl_Clk_le_Prep where
 lemmas Cl_Clk_le_PrepI = Cl_Clk_le_Prep_def[THEN iffD2, rule_format]
 lemmas Cl_Clk_le_PrepE[elim] = Cl_Clk_le_Prep_def[THEN iffD1, elim_format, rule_format]
 
-lemma reach_cl_clk_le_prep [simp]: "reach tps_s s \<Longrightarrow> Cl_Clk_le_Prep s cl"
+lemma reach_cl_clk_le_prep [simp]: "reach tps s \<Longrightarrow> Cl_Clk_le_Prep s cl"
 proof(induction s rule: reach.induct)
   case (reach_init s)
-  then show ?case by (auto simp add: Cl_Clk_le_Prep_def tps_s_defs)
+  then show ?case by (auto simp add: Cl_Clk_le_Prep_def tps_defs)
 next
   case (reach_trans s e s')
   then show ?case
@@ -1551,7 +1543,7 @@ qed
 lemma cl_clock_monotonic_WCommit:
   assumes
     "state_trans s (WCommit cl kv_map cts sn u'' clk mmap) s'"
-    "reach tps_s s"
+    "reach tps s"
   shows "cl_clock (cls s' cl) > (cl_clock (cls s cl))"
   using assms
 proof -
@@ -1571,7 +1563,7 @@ proof -
 qed
 
 lemma cl_clock_monotonic:
-  "state_trans s e s' \<Longrightarrow> reach tps_s s \<Longrightarrow> cl_clock (cls s' cl) \<ge> cl_clock (cls s cl)"
+  "state_trans s e s' \<Longrightarrow> reach tps s \<Longrightarrow> cl_clock (cls s' cl) \<ge> cl_clock (cls s cl)"
 proof (induction e)
   case (WCommit x1 x2 x3 x4 x5 x6 x7)
   then show ?case using cl_clock_monotonic_WCommit[of s x1]
@@ -1584,11 +1576,11 @@ definition Pend_le_Clk where
 lemmas Pend_le_ClkI = Pend_le_Clk_def[THEN iffD2, rule_format]
 lemmas Pend_le_ClkE[elim] = Pend_le_Clk_def[THEN iffD1, elim_format, rule_format]
 
-lemma reach_pend_le_clk [simp]: "reach tps_s s \<Longrightarrow> Pend_le_Clk s svr"
+lemma reach_pend_le_clk [simp]: "reach tps s \<Longrightarrow> Pend_le_Clk s svr"
 proof(induction s rule: reach.induct)
   case (reach_init s)
   then show ?case
-    by (auto simp add: Pend_le_Clk_def tps_s_defs pending_wtxns_ts_def split: if_split_asm)
+    by (auto simp add: Pend_le_Clk_def tps_defs pending_wtxns_ts_def split: if_split_asm)
 next
   case (reach_trans s e s')
   then show ?case
@@ -1617,11 +1609,11 @@ definition Prep_le_Clk where
 lemmas Prep_le_ClkI = Prep_le_Clk_def[THEN iffD2, rule_format]
 lemmas Prep_le_ClkE[elim] = Prep_le_Clk_def[THEN iffD1, elim_format, rule_format]
 
-lemma reach_prep_le_clk [simp]: "reach tps_s s \<Longrightarrow> Prep_le_Clk s svr"
+lemma reach_prep_le_clk [simp]: "reach tps s \<Longrightarrow> Prep_le_Clk s svr"
 proof(induction s rule: reach.induct)
   case (reach_init s)
   then show ?case
-    by (auto simp add: Prep_le_Clk_def tps_s_defs pending_wtxns_ts_def split: if_split_asm)
+    by (auto simp add: Prep_le_Clk_def tps_defs pending_wtxns_ts_def split: if_split_asm)
 next
   case (reach_trans s e s')
   then show ?case
@@ -1650,11 +1642,11 @@ definition Pend_lt_Prep where
 lemmas Pend_lt_PrepI = Pend_lt_Prep_def[THEN iffD2, rule_format]
 lemmas Pend_lt_PrepE[elim] = Pend_lt_Prep_def[THEN iffD1, elim_format, rule_format]
 
-lemma reach_pend_lt_prep [simp]: "reach tps_s s \<Longrightarrow> Pend_lt_Prep s svr"
+lemma reach_pend_lt_prep [simp]: "reach tps s \<Longrightarrow> Pend_lt_Prep s svr"
 proof(induction s rule: reach.induct)
   case (reach_init s)
   then show ?case
-    by (auto simp add: Pend_lt_Prep_def tps_s_defs)
+    by (auto simp add: Pend_lt_Prep_def tps_defs)
 next
   case (reach_trans s e s')
   then show ?case
@@ -1668,11 +1660,11 @@ definition Lst_le_Clk where
 lemmas Lst_le_ClkI = Lst_le_Clk_def[THEN iffD2, rule_format]
 lemmas Lst_le_ClkE[elim] = Lst_le_Clk_def[THEN iffD1, elim_format, rule_format]
 
-lemma reach_lst_le_clk [simp, dest]: "reach tps_s s \<Longrightarrow> Lst_le_Clk s k"
+lemma reach_lst_le_clk [simp, dest]: "reach tps s \<Longrightarrow> Lst_le_Clk s k"
 proof(induction s rule: reach.induct)
   case (reach_init s)
   then show ?case
-  by (auto simp add: Lst_le_Clk_def tps_s_defs)
+  by (auto simp add: Lst_le_Clk_def tps_defs)
 next
   case (reach_trans s e s')
   then show ?case 
@@ -1691,11 +1683,11 @@ definition Lst_le_Pend where
 lemmas Lst_le_PendI = Lst_le_Pend_def[THEN iffD2, rule_format]
 lemmas Lst_le_PendE[elim] = Lst_le_Pend_def[THEN iffD1, elim_format, rule_format]
 
-lemma reach_lst_le_pend [simp]: "reach tps_s s \<Longrightarrow> Lst_le_Pend s svr"
+lemma reach_lst_le_pend [simp]: "reach tps s \<Longrightarrow> Lst_le_Pend s svr"
 proof(induction s rule: reach.induct)
   case (reach_init s)
   then show ?case
-  by (auto simp add: Lst_le_Pend_def tps_s_defs )
+  by (auto simp add: Lst_le_Pend_def tps_defs )
 next
   case (reach_trans s e s')
   then show ?case 
@@ -1716,7 +1708,7 @@ lemma min_pending_wtxns_monotonic:
   assumes "state_trans s e s'"
     and "pending_wtxns_ts (svr_state (svrs s k)) \<noteq> {}"
     and "pending_wtxns_ts (svr_state (svrs s' k)) \<noteq> {}"
-    and "reach tps_s s"
+    and "reach tps s"
   shows "Min (pending_wtxns_ts (svr_state (svrs s k))) \<le>
          Min (pending_wtxns_ts (svr_state (svrs s' k)))"
   using assms
@@ -1742,7 +1734,7 @@ next
 
 lemma svr_lst_monotonic:
   assumes "state_trans s e s'"
-    and "reach tps_s s"
+    and "reach tps s"
   shows "svr_lst (svrs s' svr) \<ge> svr_lst (svrs s svr)"
   using assms
   proof (induction e)
@@ -1762,10 +1754,10 @@ definition Rlst_le_Lst where
 lemmas Rlst_le_LstI = Rlst_le_Lst_def[THEN iffD2, rule_format]
 lemmas Rlst_le_LstE[elim] = Rlst_le_Lst_def[THEN iffD1, elim_format, rule_format]
 
-lemma reach_rlst_le_lst [simp]: "reach tps_s s \<Longrightarrow> Rlst_le_Lst s k"
+lemma reach_rlst_le_lst [simp]: "reach tps s \<Longrightarrow> Rlst_le_Lst s k"
 proof(induction s rule: reach.induct)
   case (reach_init s)
-  then show ?case by (auto simp add: Rlst_le_Lst_def tps_s_defs)
+  then show ?case by (auto simp add: Rlst_le_Lst_def tps_defs)
 next
   case (reach_trans s e s')
   then show ?case
@@ -1793,10 +1785,10 @@ definition Get_lst_le_Lst where
 lemmas Get_lst_le_LstI = Get_lst_le_Lst_def[THEN iffD2, rule_format]
 lemmas Get_lst_le_LstE[elim] = Get_lst_le_Lst_def[THEN iffD1, elim_format, rule_format]
 
-lemma reach_get_lst_le_lst [simp]: "reach tps_s s \<Longrightarrow> Get_lst_le_Lst s k"
+lemma reach_get_lst_le_lst [simp]: "reach tps s \<Longrightarrow> Get_lst_le_Lst s k"
 proof(induction s rule: reach.induct)
   case (reach_init s)
-  then show ?case by (auto simp add: Get_lst_le_Lst_def tps_s_defs)
+  then show ?case by (auto simp add: Get_lst_le_Lst_def tps_defs)
 next
   case (reach_trans s e s')
   then show ?case
@@ -1823,11 +1815,11 @@ definition Lst_map_le_Lst where
 lemmas Lst_map_le_LstI = Lst_map_le_Lst_def[THEN iffD2, rule_format]
 lemmas Lst_map_le_LstE[elim] = Lst_map_le_Lst_def[THEN iffD1, elim_format, rule_format]
 
-lemma reach_lst_map_le_svr_lst [simp]: "reach tps_s s \<Longrightarrow> Lst_map_le_Lst s cl k"
+lemma reach_lst_map_le_svr_lst [simp]: "reach tps s \<Longrightarrow> Lst_map_le_Lst s cl k"
 proof(induction s rule: reach.induct)
   case (reach_init s)
   then show ?case
-  by (auto simp add: Lst_map_le_Lst_def tps_s_defs)
+  by (auto simp add: Lst_map_le_Lst_def tps_defs)
 next
   case (reach_trans s e s')
   then show ?case
@@ -1858,11 +1850,11 @@ definition Prep_le_Cl_Cts where
 lemmas Prep_le_Cl_CtsI = Prep_le_Cl_Cts_def[THEN iffD2, rule_format]
 lemmas Prep_le_Cl_CtsE[elim] = Prep_le_Cl_Cts_def[THEN iffD1, elim_format, rule_format]
 
-lemma reach_prep_le_cl_cts [simp]: "reach tps_s s \<Longrightarrow> Prep_le_Cl_Cts s cl"
+lemma reach_prep_le_cl_cts [simp]: "reach tps s \<Longrightarrow> Prep_le_Cl_Cts s cl"
 proof(induction s rule: reach.induct)
   case (reach_init s)
   then show ?case
-  by (auto simp add: Prep_le_Cl_Cts_def tps_s_defs)
+  by (auto simp add: Prep_le_Cl_Cts_def tps_defs)
 next
   case (reach_trans s e s')
   then show ?case 
@@ -1889,10 +1881,10 @@ definition Lst_map_le_Get_lst where
 lemmas Lst_map_le_Get_lstI = Lst_map_le_Get_lst_def[THEN iffD2, rule_format]
 lemmas Lst_map_le_Get_lstE[elim] = Lst_map_le_Get_lst_def[THEN iffD1, elim_format, rule_format]
 
-lemma reach_lst_map_le_get_lst [simp]: "reach tps_s s \<Longrightarrow> Lst_map_le_Get_lst s cl k"
+lemma reach_lst_map_le_get_lst [simp]: "reach tps s \<Longrightarrow> Lst_map_le_Get_lst s cl k"
 proof(induction s rule: reach.induct)
   case (reach_init s)
-  then show ?case by (auto simp add: Lst_map_le_Get_lst_def tps_s_defs)
+  then show ?case by (auto simp add: Lst_map_le_Get_lst_def tps_defs)
 next
   case (reach_trans s e s')
   then show ?case
@@ -1982,7 +1974,7 @@ lemmas circular_defs = Fresh_rd_notin_other_rs_def Once_in_rs_def
 
 lemma lst_map_monotonic_dep:
   assumes "state_trans s e s'"
-    and "reach tps_s s"
+    and "reach tps s"
     and "\<And>cl k. Lst_map_le_Rlst s cl k"
   shows "lst_map (cls s cl) k \<le> lst_map (cls s' cl) k"
   using assms
@@ -2002,7 +1994,7 @@ qed (auto simp add: tps_trans_defs)
 (*** The start of dependent lemmas/invariants ***)
 lemma lst_map_min_monotonic_dep:
   assumes "state_trans s e s'"
-    and "reach tps_s s"
+    and "reach tps s"
     and "\<And>cl k. Lst_map_le_Rlst s cl k"
   shows "Min (range (lst_map (cls s cl))) \<le> Min (range (lst_map (cls s' cl)))"
   using assms lst_map_monotonic_dep[of s] Finite_Lst_map_Ran_def[of s] Finite_Lst_map_Ran_def[of s']
@@ -2010,7 +2002,7 @@ lemma lst_map_min_monotonic_dep:
   by (meson Min.coboundedI dual_order.trans rangeI)
 
 lemma reach_gst_lt_cl_cts_dep:
-  assumes "reach tps_s s"                                   
+  assumes "reach tps s"                                   
     "Gst_le_Pend_t s cl"
   shows "Gst_lt_Cl_Cts s cl k"
   using assms
@@ -2022,7 +2014,7 @@ lemma reach_gst_lt_cl_cts_dep:
   done
 
 lemma reach_gst_le_pd_dep: 
-  assumes "reach tps_s s"
+  assumes "reach tps s"
     "\<And>k. Gst_le_Min_Lst_map s k"
   shows "Gst_le_Pend_t s cl"
   using assms Gst_le_Min_Lst_map_def[of s cl] Lst_map_le_Lst_def[of s cl] Lst_le_Pend_def[of s]
@@ -2031,17 +2023,17 @@ lemma reach_gst_le_pd_dep:
   by (meson Min.coboundedI dual_order.trans rangeI reach_finite_lst_map_ran)
 
 lemma reach_all_circular:
-  "reach tps_s s \<Longrightarrow> (\<forall>cl k. Fresh_rd_notin_other_rs s cl k) \<and> (\<forall>k t. Once_in_rs s k t) \<and>
+  "reach tps s \<Longrightarrow> (\<forall>cl k. Fresh_rd_notin_other_rs s cl k) \<and> (\<forall>k t. Once_in_rs s k t) \<and>
     (\<forall>cl k. Lst_map_le_Rlst s cl k) \<and> (\<forall>cl. Gst_le_Min_Lst_map s cl)"
 proof(induction s rule: reach.induct)
   case (reach_init s)
-  then show ?case by (auto simp add: circular_defs tps_s_defs)
+  then show ?case by (auto simp add: circular_defs tps_defs)
 next
   case (reach_trans s e s')
   then show ?case
   proof (intro allI conjI; elim conjE)
     fix cl k
-    assume a: "tps_s: s \<midarrow>e\<rightarrow> s'" "reach tps_s s" "\<forall>cl. Gst_le_Min_Lst_map s cl"
+    assume a: "tps: s \<midarrow>e\<rightarrow> s'" "reach tps s" "\<forall>cl. Gst_le_Min_Lst_map s cl"
       "\<forall>cl k. Fresh_rd_notin_other_rs s cl k"
     then have "Fresh_rd_notin_other_rs s cl k" by simp
     then show "Fresh_rd_notin_other_rs s' cl k" using a
@@ -2073,7 +2065,7 @@ next
     qed (auto simp add: Fresh_rd_notin_other_rs_def tps_trans_defs split: txn_state.split)
   next
     fix k t
-    assume a: "tps_s: s \<midarrow>e\<rightarrow> s'" "reach tps_s s" "\<forall>cl k. Fresh_rd_notin_other_rs s cl k"
+    assume a: "tps: s \<midarrow>e\<rightarrow> s'" "reach tps s" "\<forall>cl k. Fresh_rd_notin_other_rs s cl k"
       "\<forall>k t. Once_in_rs s k t"
     then have "Once_in_rs s k t" by simp
     then show "Once_in_rs s' k t" using a
@@ -2089,7 +2081,7 @@ next
     qed (auto simp add: Once_in_rs_def tps_trans_defs)
   next
     fix cl k
-    assume a: "tps_s: s \<midarrow>e\<rightarrow> s'" "reach tps_s s" "\<forall>k t. Once_in_rs s k t"
+    assume a: "tps: s \<midarrow>e\<rightarrow> s'" "reach tps s" "\<forall>k t. Once_in_rs s k t"
       "\<forall>cl k. Lst_map_le_Rlst s cl k"
     then have "Lst_map_le_Rlst s cl k" by simp
     then show "Lst_map_le_Rlst s' cl k" using a
@@ -2126,7 +2118,7 @@ next
     qed (auto simp add: Lst_map_le_Rlst_def tps_trans_defs)
   next
     fix k
-    assume a: "tps_s: s \<midarrow>e\<rightarrow> s'" "reach tps_s s" "\<forall>cl k. Lst_map_le_Rlst s cl k"
+    assume a: "tps: s \<midarrow>e\<rightarrow> s'" "reach tps s" "\<forall>cl k. Lst_map_le_Rlst s cl k"
       "\<forall>k. Gst_le_Min_Lst_map s k"
     then have "Gst_le_Min_Lst_map s k" by simp
     then show "Gst_le_Min_Lst_map s' k" using a
@@ -2146,39 +2138,39 @@ qed
 (*** The end of dependent lemmas/invariants ***)
 
 lemma reach_fresh_rd_notin_other_rs [simp]:
-  "reach tps_s s \<Longrightarrow> Fresh_rd_notin_other_rs s cl k"
+  "reach tps s \<Longrightarrow> Fresh_rd_notin_other_rs s cl k"
   by (simp add: reach_all_circular)
 
 lemma reach_once_in_rs [simp]:
-  "reach tps_s s \<Longrightarrow> Once_in_rs s k t"
+  "reach tps s \<Longrightarrow> Once_in_rs s k t"
   by (simp add: reach_all_circular)
 
 lemma reach_lst_map_le_rlst [simp]:
-  "reach tps_s s \<Longrightarrow> Lst_map_le_Rlst s cl k"
+  "reach tps s \<Longrightarrow> Lst_map_le_Rlst s cl k"
   by (simp add: reach_all_circular)
 
 lemma reach_gst_le_min_lst_map [simp]:
-  "reach tps_s s \<Longrightarrow> Gst_le_Min_Lst_map s k"
+  "reach tps s \<Longrightarrow> Gst_le_Min_Lst_map s k"
   by (simp add: reach_all_circular)
 
 lemma lst_map_monotonic:
   assumes "state_trans s e s'"
-    and "reach tps_s s"
+    and "reach tps s"
   shows "lst_map (cls s cl) k \<le> lst_map (cls s' cl) k"
   using assms
   by (simp add: reach_all_circular lst_map_monotonic_dep)
 
 lemma lst_map_min_monotonic:
   assumes "state_trans s e s'"
-    and "reach tps_s s"
+    and "reach tps s"
   shows "Min (range (lst_map (cls s cl))) \<le> Min (range (lst_map (cls s' cl)))"
   using assms
   by (simp add: reach_all_circular lst_map_min_monotonic_dep)
 
-lemma reach_gst_lt_cl_cts [simp]: "reach tps_s s \<Longrightarrow> Gst_lt_Cl_Cts s cl k"
+lemma reach_gst_lt_cl_cts [simp]: "reach tps s \<Longrightarrow> Gst_lt_Cl_Cts s cl k"
   by (simp add: reach_all_circular reach_gst_le_pd_dep reach_gst_lt_cl_cts_dep)
 
-lemma reach_gst_le_pd [simp]: "reach tps_s s \<Longrightarrow> Gst_le_Pend_t s cl"
+lemma reach_gst_le_pd [simp]: "reach tps s \<Longrightarrow> Gst_le_Pend_t s cl"
   by (simp add: reach_all_circular reach_gst_le_pd_dep)
 
 definition Gst_lt_Cts where
@@ -2188,11 +2180,11 @@ definition Gst_lt_Cts where
 lemmas Gst_lt_CtsI = Gst_lt_Cts_def[THEN iffD2, rule_format]
 lemmas Gst_lt_CtsE[elim] = Gst_lt_Cts_def[THEN iffD1, elim_format, rule_format]
 
-lemma reach_gst_lt_cts [simp]: "reach tps_s s \<Longrightarrow> Gst_lt_Cts s cl"
+lemma reach_gst_lt_cts [simp]: "reach tps s \<Longrightarrow> Gst_lt_Cts s cl"
 proof(induction s rule: reach.induct)
   case (reach_init s)
   then show ?case
-  by (auto simp add: Gst_lt_Cts_def tps_s_defs)
+  by (auto simp add: Gst_lt_Cts_def tps_defs)
 next
   case (reach_trans s e s')
   then show ?case 
@@ -2224,7 +2216,7 @@ qed
 
 lemma gst_monotonic:
   assumes "state_trans s e s'"
-    and "reach tps_s s"
+    and "reach tps s"
   shows "gst (cls s' cl) \<ge> gst (cls s cl)"
   using assms using Gst_le_Min_Lst_map_def[of s]
   by (induction e) (auto simp add: tps_trans_defs)
@@ -2236,10 +2228,10 @@ definition Rtxn_rts_le_Gst where
 lemmas Rtxn_rts_le_GstI = Rtxn_rts_le_Gst_def[THEN iffD2, rule_format]
 lemmas Rtxn_rts_le_GstE[elim] = Rtxn_rts_le_Gst_def[THEN iffD1, elim_format, rule_format]
 
-lemma reach_rtxn_rts_le_gst [simp]: "reach tps_s s \<Longrightarrow> Rtxn_rts_le_Gst s cl"
+lemma reach_rtxn_rts_le_gst [simp]: "reach tps s \<Longrightarrow> Rtxn_rts_le_Gst s cl"
 proof(induction s rule: reach.induct)
   case (reach_init s)
-  then show ?case by (auto simp add: Rtxn_rts_le_Gst_def tps_s_defs)
+  then show ?case by (auto simp add: Rtxn_rts_le_Gst_def tps_defs)
 next
   case (reach_trans s e s')
   then show ?case 
@@ -2249,7 +2241,6 @@ next
       by (meson Gst_le_Min_Lst_map_def order.trans reach_gst_le_min_lst_map reach_gst_lt_cl_cts)
   qed (auto simp add: Rtxn_rts_le_Gst_def tps_trans_defs)
 qed
-
 
 subsection \<open>Commit Timestamps Order Invariants\<close>
 
@@ -2261,11 +2252,11 @@ definition CO_Tid where
 lemmas CO_TidI = CO_Tid_def[THEN iffD2, rule_format]
 lemmas CO_TidE[elim] = CO_Tid_def[THEN iffD1, elim_format, rule_format]
 
-lemma reach_co_tid[simp]: "reach tps_s s \<Longrightarrow> CO_Tid s cl"
+lemma reach_co_tid[simp]: "reach tps s \<Longrightarrow> CO_Tid s cl"
 proof(induction s rule: reach.induct)
   case (reach_init s)
   then show ?case
-    by (auto simp add: CO_Tid_def tps_s_defs)
+    by (auto simp add: CO_Tid_def tps_defs)
 next
   case (reach_trans s e s')
   then show ?case
@@ -2288,1829 +2279,70 @@ next
   qed (auto simp add: CO_Tid_def tps_trans_defs split: txn_state.split_asm)
 qed
 
-definition CO_Distinct where
-  "CO_Distinct s k \<longleftrightarrow> distinct (cts_order s k)"
 
-lemmas CO_DistinctI = CO_Distinct_def[THEN iffD2, rule_format]
-lemmas CO_DistinctE[elim] = CO_Distinct_def[THEN iffD1, elim_format, rule_format]
-
-lemma reach_co_distinct [simp]: "reach tps_s s \<Longrightarrow> CO_Distinct s k"
-proof(induction s rule: reach.induct)
-  case (reach_init s)
-  then show ?case
-    by (auto simp add: CO_Distinct_def tps_s_defs)
-next
-  case (reach_trans s e s')
-  then show ?case
-  proof (induction e)
-    case (WCommit x1 x2 x3 x4 x5 x6 x7)
-    then show ?case apply (auto simp add: CO_Distinct_def tps_trans_all_defs distinct_insort)
-      by (metis (no_types, lifting) CO_Tid_def less_irrefl_nat reach_co_tid txn_state.simps(18))
-  qed (simp_all add: CO_Distinct_def tps_trans_defs)
-qed
-
-definition CO_Tn_is_Cmt_Abs where
-  "CO_Tn_is_Cmt_Abs s k \<longleftrightarrow> (\<forall>n cl. Tn (Tn_cl n cl) \<in> set (cts_order s k) \<longrightarrow>
-    (\<exists>cts sts lst v rs. svr_state (svrs s k) (Tn (Tn_cl n cl)) = Commit cts sts lst v rs) \<or> 
-    ((\<exists>pd ts v. svr_state (svrs s k) (Tn (Tn_cl n cl)) = Prep pd ts v) \<and> 
-     (\<exists>cts kv_map. cl_state (cls s cl) = WtxnCommit cts kv_map \<and> 
-      cl_sn (cls s cl) = n \<and> k \<in> dom kv_map)))"
-
-lemmas CO_Tn_is_Cmt_AbsI = CO_Tn_is_Cmt_Abs_def[THEN iffD2, rule_format]
-lemmas CO_Tn_is_Cmt_AbsE[elim] = CO_Tn_is_Cmt_Abs_def[THEN iffD1, elim_format, rule_format]
-
-lemma reach_co_tn_is_cmt_abs [simp]: "reach tps_s s \<Longrightarrow> CO_Tn_is_Cmt_Abs s k"
-proof(induction s rule: reach.induct)
-  case (reach_init s)
-  then show ?case
-    by (auto simp add: CO_Tn_is_Cmt_Abs_def tps_s_defs)
-next
-  case (reach_trans s e s')
-  then show ?case
-  proof (induction e)
-    case (RInvoke x1 x2 x3 x4)
-    then show ?case apply (simp add: CO_Tn_is_Cmt_Abs_def tps_trans_defs)
-      by (metis txn_state.distinct(5))
-  next
-    case (Read x1 x2 x3 x4 x5 x6 x7)
-    then show ?case apply (simp add: CO_Tn_is_Cmt_Abs_def tps_trans_defs)
-      by (metis txn_state.distinct(9))
-  next
-    case (RDone x1 x2 x3 x4 x5)
-    then show ?case apply (simp add: CO_Tn_is_Cmt_Abs_def tps_trans_defs)
-      by (metis txn_state.distinct(9))
-  next
-    case (WInvoke x1 x2 x3 x4)
-    then show ?case apply (simp add: CO_Tn_is_Cmt_Abs_def tps_trans_defs)
-      by (metis txn_state.distinct(5))
-  next
-    case (WCommit x1 x2 x3 x4 x5 x6 x7)
-    then show ?case apply (simp add: CO_Tn_is_Cmt_Abs_def tps_trans_all_defs set_insort_key)
-      by (smt (verit) domIff is_prepared.elims(2) option.discI txn_state.distinct(11))
-  next
-    case (WDone x1 x2 x3 x4 x5)
-    then show ?case apply (simp add: CO_Tn_is_Cmt_Abs_def tps_trans_defs)
-      by (metis (no_types, lifting) txn_state.inject(3))
-  next
-    case (RegR x1 x2 x3 x4 x5 x6 x7)
-    then show ?case apply (simp add: CO_Tn_is_Cmt_Abs_def tps_trans_defs)
-      by (metis add_to_readerset_commit' add_to_readerset_prep_inv)
-  next
-    case (PrepW x1 x2 x3 x4 x5)
-    then show ?case apply (simp add: CO_Tn_is_Cmt_Abs_def tps_trans_defs)
-      by (metis ver_state.distinct(3))
-  next
-    case (CommitW x1 x2 x3 x4 x5 x6 x7)
-    then show ?case apply (simp add: CO_Tn_is_Cmt_Abs_def tps_trans_defs)
-      by (smt (z3) fun_upd_apply txn_state.simps(19) ver_state.simps(10))
-  qed
-qed
-
-definition CO_is_Cmt_Abs where
-  "CO_is_Cmt_Abs s k \<longleftrightarrow> (\<forall>t. t \<in> set (cts_order s k) \<longrightarrow>
-    (\<exists>cts sts lst v rs. svr_state (svrs s k) t = Commit cts sts lst v rs) \<or> 
-    ((\<exists>pd ts v. svr_state (svrs s k) t = Prep pd ts v) \<and> 
-     (\<exists>cts kv_map. cl_state (cls s (get_cl_w t)) = WtxnCommit cts kv_map \<and> k \<in> dom kv_map)))"
-
-lemmas CO_is_Cmt_AbsI = CO_is_Cmt_Abs_def[THEN iffD2, rule_format]
-lemmas CO_is_Cmt_AbsE[elim] = CO_is_Cmt_Abs_def[THEN iffD1, elim_format, rule_format]
-
-lemma reach_co_is_cmt_abs [simp]: "reach tps_s s \<Longrightarrow> CO_is_Cmt_Abs s k"
-  apply (simp add: CO_is_Cmt_Abs_def)
-  apply rule subgoal for t apply (cases t)
-    apply (metis Init_Ver_Inv_def reach_init_ver_inv)
-    by (smt CO_Tn_is_Cmt_Abs_def get_cl_w.simps(2) reach_co_tn_is_cmt_abs txid0.collapse).
-
-definition CO_not_No_Ver where
-  "CO_not_No_Ver s k \<longleftrightarrow> (\<forall>t \<in> set (cts_order s k). svr_state (svrs s k) t \<noteq> No_Ver)"
-
-lemmas CO_not_No_VerI = CO_not_No_Ver_def[THEN iffD2, rule_format]
-lemmas CO_not_No_VerE[elim] = CO_not_No_Ver_def[THEN iffD1, elim_format, rule_format]
-
-lemma reach_co_not_no_ver [simp]: "reach tps_s s \<Longrightarrow> CO_not_No_Ver s k"
-  apply (auto simp add: CO_not_No_Ver_def)
-  by (metis CO_is_Cmt_Abs_def reach_co_is_cmt_abs ver_state.distinct(1) ver_state.distinct(3))
-
-definition CO_has_Cts where
-  "CO_has_Cts s k \<longleftrightarrow> (\<forall>t \<in> set (cts_order s k). \<exists>cts. wtxn_cts s t = Some cts)"
-
-lemmas CO_has_CtsI = CO_has_Cts_def[THEN iffD2, rule_format]
-lemmas CO_has_CtsE[elim] = CO_has_Cts_def[THEN iffD1, elim_format, rule_format]
-
-lemma reach_co_has_cts [simp]: "reach tps_s s \<Longrightarrow> CO_has_Cts s k"
-  apply (simp add: CO_has_Cts_def)
-  apply rule subgoal for t apply (cases t)
-    using Init_Ver_Inv_def Wtxn_State_Cts_def[of s k] reach_svr_state_cts
-    apply (metis reach_init_ver_inv)
-    by (metis CO_Tn_is_Cmt_Abs_def[of s] Wtxn_State_Cts_def WtxnCommit_Wtxn_Cts_def
-        reach_co_tn_is_cmt_abs reach_svr_state_cts reach_wtxncommit_wtxn_cts txid0.exhaust).
-
-definition Committed_Abs_Tn_in_CO where
-  "Committed_Abs_Tn_in_CO s k \<longleftrightarrow> (\<forall>n cl.
-    (\<exists>cts sts lst v rs. svr_state (svrs s k) (Tn (Tn_cl n cl)) = Commit cts sts lst v rs) \<or> 
-    ((\<exists>pd ts v. svr_state (svrs s k) (Tn (Tn_cl n cl)) = Prep pd ts v) \<and> 
-     (\<exists>cts kv_map. cl_state (cls s cl) = WtxnCommit cts kv_map \<and> cl_sn (cls s cl) = n)) \<longrightarrow>
-    Tn (Tn_cl n cl) \<in> set (cts_order s k))"
-
-lemmas Committed_Abs_Tn_in_COI = Committed_Abs_Tn_in_CO_def[THEN iffD2, rule_format]
-lemmas Committed_Abs_Tn_in_COE[elim] = Committed_Abs_Tn_in_CO_def[THEN iffD1, elim_format, rule_format]
-
-lemma reach_cmt_abs_tn_in_co [simp]: "reach tps_s s \<Longrightarrow> Committed_Abs_Tn_in_CO s k"
-proof(induction s rule: reach.induct)
-  case (reach_init s)
-  then show ?case
-    by (auto simp add: Committed_Abs_Tn_in_CO_def tps_s_defs split: if_split_asm)
-next
-  case (reach_trans s e s')
-  then show ?case
-  proof (induction e)
-    case (Read x1 x2 x3 x4 x5 x6 x7)
-    then show ?case apply (simp add: Committed_Abs_Tn_in_CO_def tps_trans_defs)
-      by (metis txn_state.distinct(9) txn_state.simps(17))
-  next
-    case (WCommit x1 x2 x3 x4 x5 x6 x7)
-    then show ?case apply (simp add: Committed_Abs_Tn_in_CO_def tps_trans_all_defs set_insort_key)
-      by (metis (no_types, lifting) Cl_Prep_Inv_def domIff reach_cl_prep_inv ver_state.distinct(1))
-  next
-    case (RegR x1 x2 x3 x4 x5 x6 x7)
-    then show ?case apply (simp add: Committed_Abs_Tn_in_CO_def tps_trans_defs)
-      by (smt (verit) add_to_readerset_commit add_to_readerset_prep_inv)
-  next
-    case (PrepW x1 x2 x3 x4 x5)
-    then show ?case apply (simp add: Committed_Abs_Tn_in_CO_def tps_trans_defs)
-      by (metis get_cl_w.simps(2) txn_state.distinct(11) txid0.collapse)
-  qed (auto simp add: Committed_Abs_Tn_in_CO_def tps_trans_defs)
-qed
-
-definition Committed_Abs_in_CO where
-  "Committed_Abs_in_CO s k \<longleftrightarrow> (\<forall>t.
-    (\<exists>cts sts lst v rs. svr_state (svrs s k) t = Commit cts sts lst v rs) \<or> 
-    ((\<exists>pd ts v. svr_state (svrs s k) t = Prep pd ts v) \<and>
-     (\<exists>cts kv_map. cl_state (cls s (get_cl_w t)) = WtxnCommit cts kv_map)) \<longrightarrow>
-    t \<in> set (cts_order s k))"
-
-lemmas Committed_Abs_in_COI = Committed_Abs_in_CO_def[THEN iffD2, rule_format]
-lemmas Committed_Abs_in_COE[elim] = Committed_Abs_in_CO_def[THEN iffD1, elim_format, rule_format]
-
-lemma reach_cmt_abs_in_co [simp]: "reach tps_s s \<Longrightarrow> Committed_Abs_in_CO s k"
-  apply (simp add: Committed_Abs_in_CO_def)
-  apply rule subgoal for t apply (cases t, blast)
-  by (metis Prep_is_Curr_wt_def[of s k] Committed_Abs_Tn_in_CO_def get_cl_w.simps(2) txid0.collapse
-      get_sn_w.simps(2) is_prepared.simps(1) reach_cmt_abs_tn_in_co reach_prep_is_curr_wt).
-
-definition CO_Sorted where
-  "CO_Sorted s k \<longleftrightarrow> (\<forall>i. \<forall>i' < length (cts_order s k).
-    i < i' \<longrightarrow> the (wtxn_cts s (cts_order s k ! i)) \<le> the (wtxn_cts s (cts_order s k ! i')))"
-
-lemmas CO_SortedI = CO_Sorted_def[THEN iffD2, rule_format]
-lemmas CO_SortedE[elim] = CO_Sorted_def[THEN iffD1, elim_format, rule_format]
-
-lemma reach_co_sorted [simp]: "reach tps_s s \<Longrightarrow> CO_Sorted s k"
-proof(induction s rule: reach.induct)
-  case (reach_init s)
-  then show ?case by (auto simp add: CO_Sorted_def tps_s_defs)
-next
-  case (reach_trans s e s')
-  then show ?case 
-  proof (induction e)
-    case (WCommit x1 x2 x3 x4 x5 x6 x7)
-    then have indom: "k \<in> dom x2 \<Longrightarrow> cts_order s' k = cts_order s k @ [get_wtxn s x1]"
-      apply (auto simp add: tps_trans_all_defs) (* CONTINUE! *) sorry
-    have nindom: "k \<notin> dom x2 \<Longrightarrow> cts_order s' k = cts_order s k" using WCommit
-      by (auto simp add: tps_trans_all_defs)
-    then show ?case using WCommit indom nindom
-      apply (cases "k \<in> dom x2", auto)
-      subgoal apply (auto simp add: CO_Sorted_def tps_trans_defs)
-      (*apply (cases "x2 k", auto)*) sorry
-      sorry
-  qed (auto simp add: CO_Sorted_def tps_trans_defs)
-qed
-
-lemma T0_min_unique_ts:
-  assumes "reach tps_s s"
-  shows "unique_ts (wtxn_cts s) t \<ge> unique_ts (wtxn_cts s) T0"
-  using assms Wtxn_Cts_T0_def[of s]
-  by (auto simp add: unique_ts_def less_eq_prod_def)
-
-definition T0_First_in_CO where
-  "T0_First_in_CO s k \<longleftrightarrow> cts_order s k ! 0 = T0"
-
-lemmas T0_First_in_COI = T0_First_in_CO_def[THEN iffD2, rule_format]
-lemmas T0_First_in_COE[elim] = T0_First_in_CO_def[THEN iffD1, elim_format, rule_format]
-
-lemma reach_t0_first_in_co [simp, dest]: "reach tps_s s \<Longrightarrow> T0_First_in_CO s k"
-proof(induction s rule: reach.induct)
-  case (reach_init s)
-  then show ?case
-    by (auto simp add: T0_First_in_CO_def tps_s_defs)
-next
-  case (reach_trans s e s')
-  then show ?case
-  proof (induction e)
-    case (WCommit x1 x2 x3 x4 x5 x6 x7)
-    then show ?case apply (auto simp add: T0_First_in_CO_def tps_trans_all_defs)
-      using T0_min_unique_ts[of s] T0_in_CO_def[of s] append_Cons empty_iff
-        empty_set neq_Nil_conv nth_Cons_0 reach_t0_in_co sorry (* Continue here! *)
-  qed (auto simp add: T0_First_in_CO_def tps_trans_all_defs)
-qed
-
-
-subsection \<open>Simulation realtion lemmas\<close>
-
-lemma kvs_of_s_init:
-  "kvs_of_s (state_init) = (\<lambda>k. [\<lparr>v_value = undefined, v_writer = T0, v_readerset = {}\<rparr>])"
-  by (simp add: kvs_of_s_defs tps_s_defs)
-
-lemma kvs_of_s_inv:
-  assumes "state_trans s e s'"
-    and "reach tps_s s"
-    and "\<not>commit_ev e"
-  shows "kvs_of_s s' = kvs_of_s s"
-  using assms(1, 3)
-proof (induction e)
-  case (WDone cl kv_map)    \<comment> \<open>write transaction already in abstract state, now just added to svr\<close>
-  then show ?case 
-    apply (auto simp add: tps_trans_defs)
-    apply (auto simp add: kvs_of_s_defs tps_trans_defs)
-    apply (intro ext)
-    apply (auto split: ver_state.split)
-    subgoal for cts k t cts' sts' lst' v' rs' t'
-      apply (thin_tac "X = Y" for X Y)
-      apply (cases "get_sn t' = cl_sn (cls s (get_cl t'))", auto)
-      using assms(2) Fresh_wr_notin_rs_def reach_fresh_wr_notin_rs
-      by (smt insert_commute insert_compr mem_Collect_eq not_None_eq singleton_conv2 txid0.collapse).
-next
-  case (RegR svr t t_wr gst_ts)
-  then show ?case       \<comment> \<open>extends readerset; ok since committed reads remain the same\<close>
-    by (auto 3 4 simp add: kvs_of_s_defs tps_trans_defs add_to_readerset_def split: ver_state.split)
-next
-  case (PrepW svr t v)  \<comment> \<open>goes to Prep state; not yet added to abstract state (client not committed)\<close>
-  then show ?case using assms(2) CO_not_No_Ver_def reach_co_not_no_ver
-    apply (auto simp add: kvs_of_s_defs, intro ext)
-    by (auto simp add: tps_trans_defs split: ver_state.split)
-next
-  case (CommitW svr t v cts)   \<comment> \<open>goes to Commit state; ok: no change\<close>
-  then show ?case  
-    by (fastforce simp add: kvs_of_s_defs tps_trans_defs split: ver_state.split)
-qed (auto 3 4 simp add: kvs_of_s_defs tps_trans_defs split: ver_state.split)
-
-(* two auto 3 4 are SLOW *)
-
-subsection \<open>Transaction ID Freshness\<close>
-
-definition Sqn_Inv_nc where
-  "Sqn_Inv_nc s cl \<longleftrightarrow> (\<forall>cts kv_map. cl_state (cls s cl) \<noteq> WtxnCommit cts kv_map
-     \<longrightarrow> (\<forall>m \<in> get_sqns (kvs_of_s s) cl. m < cl_sn (cls s cl)))"
-
-lemmas Sqn_Inv_ncI = Sqn_Inv_nc_def[THEN iffD2, rule_format]
-lemmas Sqn_Inv_ncE[elim] = Sqn_Inv_nc_def[THEN iffD1, elim_format, rule_format]
-
-lemma reach_sql_inv_nc [simp]: "reach tps_s s \<Longrightarrow> Sqn_Inv_nc s cl"
-proof(induction s rule: reach.induct)
-  case (reach_init s)
-  then show ?case
-    by (auto simp add: Sqn_Inv_nc_def tps_s_def kvs_of_s_init get_sqns_old_def txid_defs)
-next
-  case (reach_trans s e s')
-  then show ?case using kvs_of_s_inv[of s e s']
-  proof (induction e)
-    case (RDone x1 x2 x3 x4 x5)
-    hence sqn_added: "get_sqns (kvs_of_s s') x1 = get_sqns (kvs_of_s s) x1 \<union> {cl_sn (cls s x1)}" sorry
-    from RDone have "cl \<noteq> x1 \<longrightarrow> get_sqns (kvs_of_s s') cl = get_sqns (kvs_of_s s) cl"
-      apply (simp add: read_done_def read_done_U_def) sorry
-    then show ?case using RDone sqn_added by (auto simp add: Sqn_Inv_nc_def tps_trans_defs)
-  next
-    case (WCommit x1 x2 x3 x4 x5 x6 x7)
-    then show ?case apply (simp add: Sqn_Inv_nc_def tps_trans_defs) sorry
-  next
-    case (WDone x1 x2 x3 x4 x5)
-    then show ?case apply (simp add: Sqn_Inv_nc_def tps_trans_defs)
-      by (metis less_SucI nat.discI txn_state.inject(3))
-  qed (auto simp add: Sqn_Inv_nc_def tps_trans_defs)
-qed
-
-definition Sqn_Inv_c where
-  "Sqn_Inv_c s cl \<longleftrightarrow> (\<forall>cts kv_map. cl_state (cls s cl) = WtxnCommit cts kv_map
-     \<longrightarrow> (\<forall>m \<in> get_sqns (kvs_of_s s) cl. m \<le> cl_sn (cls s cl)))"
-
-lemmas Sqn_Inv_cI = Sqn_Inv_c_def[THEN iffD2, rule_format]
-lemmas Sqn_Inv_cE[elim] = Sqn_Inv_c_def[THEN iffD1, elim_format, rule_format]
-
-lemma reach_sql_inv_c [simp]: "reach tps_s s \<Longrightarrow> Sqn_Inv_c s cl"
-proof(induction s rule: reach.induct)
-  case (reach_init s)
-  then show ?case
-    by (auto simp add: Sqn_Inv_c_def tps_s_defs)
-next
-  case (reach_trans s e s')
-  then show ?case using kvs_of_s_inv[of s e s']
-  proof (induction e)
-    case (RDone x1 x2 x3 x4 x5)
-    then show ?case apply (auto simp add: Sqn_Inv_c_def)
-      by (metis (full_types) Sqn_Inv_nc_def gt_ex nless_le reach.reach_trans reach_sql_inv_nc
-          reach_trans.hyps(1) txn_state.inject(3))+
-  next
-    case (WCommit x1 x2 x3 x4 x5 x6 x7)
-    then show ?case apply (simp add: Sqn_Inv_c_def)
-      by (metis Sqn_Inv_nc_def less_or_eq_imp_le reach.reach_trans reach_sql_inv_nc
-          reach_trans.hyps(1) txn_state.inject(3))
-  qed (auto simp add: Sqn_Inv_c_def tps_trans_defs)
-qed
-
-lemma t_is_fresh:
-  assumes "Sqn_Inv_c s cl" and "Sqn_Inv_nc s cl"
-    and "cl_state (cls s cl) \<in> {WtxnPrep kv_map, RtxnInProg cclk keys kv_map}"
-  shows "get_txn s cl \<in> next_txids (kvs_of_s s) cl"
-  using assms by (auto simp add: kvs_of_s_defs next_txids_def)
-
-subsection \<open>Kvt_map values of read_done\<close>
-definition Rtxn_IdleK_notin_rs where
-  "Rtxn_IdleK_notin_rs s cl \<longleftrightarrow> (\<forall>k cclk keys kv_map t cts sts lst v rs.
-    cl_state (cls s cl) = RtxnInProg cclk keys kv_map \<and> k \<notin> keys \<and>
-    svr_state (svrs s k) t = Commit cts sts lst v rs \<longrightarrow> rs (get_txn s cl) = None)"
-
-lemmas Rtxn_IdleK_notin_rsI = Rtxn_IdleK_notin_rs_def[THEN iffD2, rule_format]
-lemmas Rtxn_IdleK_notin_rsE[elim] = Rtxn_IdleK_notin_rs_def[THEN iffD1, elim_format, rule_format]
-
-lemma reach_rtxn_idle_k_notin_rs [simp]: "reach tps_s s \<Longrightarrow> Rtxn_IdleK_notin_rs s cl"
-proof(induction s rule: reach.induct)
-  case (reach_init s)
-  then show ?case by (auto simp add: Rtxn_IdleK_notin_rs_def tps_s_defs)
-next
-  case (reach_trans s e s')
-  then show ?case 
-  proof (induction e)
-    case (RInvoke x1 x2 x3 x4)
-    then show ?case apply (auto simp add: Rtxn_IdleK_notin_rs_def tps_trans_defs)
-      using Fresh_wr_notin_rs_def[of s]
-      by (metis insertCI reach_fresh_wr_notin_rs)
-  next
-    case (RegR x1 x2 x3 x4 x5 x6 x7)
-    then show ?case 
-      by (auto simp add: Rtxn_IdleK_notin_rs_def tps_trans_defs add_to_readerset_def
-               split: ver_state.split)
-  qed (auto simp add: Rtxn_IdleK_notin_rs_def tps_trans_defs, blast?)
-qed
-
-definition Rtxn_RegK_Kvtm_Cmt_in_rs where
-  "Rtxn_RegK_Kvtm_Cmt_in_rs s cl \<longleftrightarrow> (\<forall>k cclk keys kv_map v.
-    cl_state (cls s cl) = RtxnInProg cclk keys kv_map \<and> kv_map k = Some v \<longrightarrow>
-    (\<exists>t cts sts lst rs rts rlst. svr_state (svrs s k) t = Commit cts sts lst v rs \<and> rs (get_txn s cl) = Some (rts, rlst)))"
-
-lemmas Rtxn_RegK_Kvtm_Cmt_in_rsI = Rtxn_RegK_Kvtm_Cmt_in_rs_def[THEN iffD2, rule_format]
-lemmas Rtxn_RegK_Kvtm_Cmt_in_rsE[elim] = Rtxn_RegK_Kvtm_Cmt_in_rs_def[THEN iffD1, elim_format, rule_format]
-
-lemma reach_rtxn_regk_kvtm_cmt_in_rs [simp]: "reach tps_s s \<Longrightarrow> Rtxn_RegK_Kvtm_Cmt_in_rs s cl"
-proof(induction s rule: reach.induct)
-  case (reach_init s)
-  then show ?case by (auto simp add: Rtxn_RegK_Kvtm_Cmt_in_rs_def tps_s_defs)
-next
-  case (reach_trans s e s')
-  then show ?case 
-  proof (induction e)
-    case (Read x1 x2 x3 x4 x5 x6 x7)
-    then show ?case apply (cases x7, auto simp add: Rtxn_RegK_Kvtm_Cmt_in_rs_def tps_trans_defs)
-      by (metis option.inject)
-  next
-    case (RegR x1 x2 x3 x4 x5 x6 x7)
-    then show ?case 
-      apply (auto simp add: Rtxn_RegK_Kvtm_Cmt_in_rs_def tps_trans_defs add_to_readerset_def
-                  split: ver_state.split)
-      by (metis ver_state.inject(2))
-  next
-    case (PrepW x1 x2 x3 x4 x5)
-    then show ?case apply (simp add: Rtxn_RegK_Kvtm_Cmt_in_rs_def tps_trans_defs)
-      by (metis ver_state.distinct(3))
-  next
-    case (CommitW x1 x2 x3 x4 x5 x6 x7)
-    then show ?case apply (simp add: Rtxn_RegK_Kvtm_Cmt_in_rs_def tps_trans_defs)
-      by (metis ver_state.distinct(5))
-  qed (auto simp add: Rtxn_RegK_Kvtm_Cmt_in_rs_def tps_trans_defs)
-qed
-
-subsection \<open>Timestamp relations\<close>
-
-definition Disjoint_RW where
-  "Disjoint_RW s \<longleftrightarrow> ((\<Union>k. wtxns_dom (svr_state (svrs s k))) \<inter> Tn ` (\<Union>k. wtxns_rsran (svr_state (svrs s k))) = {})"
-
-lemmas Disjoint_RWI = Disjoint_RW_def[THEN iffD2, rule_format]
-lemmas Disjoint_RWE[elim] = Disjoint_RW_def[THEN iffD1, elim_format, rule_format]
-
-lemma reach_disjoint_rw [simp]: "reach tps_s s \<Longrightarrow> Disjoint_RW s"
-proof(induction s rule: reach.induct)
-  case (reach_init s)
-  then show ?case by (auto simp add: Disjoint_RW_def tps_s_defs)
-next
-  case (reach_trans s e s')
-  then show ?case
-  proof (induction e)
-    case (RegR x1 x2 x3 x4 x5 x6 x7)
-    hence "\<And>k. wtxns_dom (svr_state (svrs s' k)) = wtxns_dom (svr_state (svrs s k))"
-      by (simp add: tps_trans_defs add_to_readerset_wtxns_dom)
-    hence "\<And>k. wtxns_rsran (svr_state (svrs s' k)) =
-      (if k = x1
-       then insert x2 (wtxns_rsran (svr_state (svrs s k)))
-       else wtxns_rsran (svr_state (svrs s k)))" using RegR
-      by (simp add: tps_trans_defs add_to_readerset_wtxns_rsran read_at_is_committed)
-    then show ?case using RegR apply (simp add: Disjoint_RW_def)
-      using Fresh_wr_notin_Wts_dom_def[of s "get_cl x2"] sorry
-  next
-    case (PrepW x1 x2 x3 x4 x5)
-    then show ?case apply (auto simp add: Disjoint_RW_def tps_trans_defs) sorry
-  next
-    case (CommitW x1 x2 x3 x4 x5 x6 x7)
-    then show ?case sorry
-  qed (auto simp add: Disjoint_RW_def tps_trans_defs)
-qed
-
-(*definition Disjoint_RW' where
-  "Disjoint_RW' s \<longleftrightarrow> (kvs_writers (kvs_of_s s) \<inter> Tn ` kvs_readers (kvs_of_s s) = {})"
-
-lemmas Disjoint_RW'I = Disjoint_RW'_def[THEN iffD2, rule_format]
-lemmas Disjoint_RW'E[elim] = Disjoint_RW'_def[THEN iffD1, elim_format, rule_format]
-
-lemma reach_disjoint_rw' [simp]: "reach tps_s s \<Longrightarrow> Disjoint_RW' s"
-proof(induction s rule: reach.induct)
-  case (reach_init s)
-  then show ?case apply (auto simp add: Disjoint_RW'_def tps_def txid_defs)
-    by (metis empty_set kvs_of_s_init list.simps(15) singletonD txid.distinct(1) version.select_convs(2))
-next
-  case (reach_trans s e s')
-  then show ?case using kvs_of_s_inv[of s e s']
-  proof (induction e)
-    case (RDone cl kv_map sn u'')
-    then show ?case apply (auto simp add: Disjoint_RW'_def tps_trans_defs txid_defs kvs_of_s_defs
-          split: ver_state.split_asm)
-      apply (metis CO_not_No_Ver_def reach_co_not_no_ver)
-      apply (metis CO_not_No_Ver_def reach_co_not_no_ver)
-      apply (metis CO_not_No_Ver_def reach_co_not_no_ver)
-        apply (metis CO_not_No_Ver_def reach_co_not_no_ver)
-      subgoal for xa xb apply (cases xb)
-        by (smt (verit) CO_Tn_is_Cmt_Abs_def[of s xa] less_irrefl_nat reach_co_tn_is_cmt_abs
-          reach_trans.hyps(2) txn_state.distinct(9) txid0.sel(1) txid0.sel(2) ver_state.distinct(5))
-      subgoal for xa xb apply (cases xb)
-        using Fresh_wr_notin_rs_def[of s] CO_Tn_is_Cmt_Abs_def[of s xa]
-      (*
-          xd \<in> set (cts_order s xc);
-          Tn xb \<in> set (cts_order s xa);
-          svr_state (svrs s xc) xd = Commit x31 x32 x33 x34;
-          svr_state (svrs s xa) (Tn xb) = Commit x31a x32a x33a x34a
-          xb \<in> x33;
-      *)
-        sorry
-      done
-  next
-    case (WCommit x1 x2 x3 x4 x5 x6 x7)
-    then show ?case sorry
-  qed (auto simp add: Disjoint_RW'_def)
-qed*)
-
-definition RO_has_rts where
-  "RO_has_rts s \<longleftrightarrow> (\<forall>t. Tn t \<in> read_only_Txs (kvs_of_s s) \<longrightarrow> (\<exists>rts. rtxn_rts s t = Some rts))"
-
-lemmas RO_has_rtsI = RO_has_rts_def[THEN iffD2, rule_format]
-lemmas RO_has_rtsE[elim] = RO_has_rts_def[THEN iffD1, elim_format, rule_format]
-
-lemma reach_ro_in_readers [simp]: "reach tps_s s \<Longrightarrow> RO_has_rts s"
-proof(induction s rule: reach.induct)
-  case (reach_init s)
-  then show ?case
-    by (auto simp add: RO_has_rts_def tps_s_defs read_only_Txs_def txid_defs kvs_of_s_defs)
-next
-  case (reach_trans s e s')
-  then show ?case using kvs_of_s_inv[of s e s']
-  proof (induction e)
-    case (RDone x1 x2 x3 x4 x5)
-    then show ?case apply (auto simp add: RO_has_rts_def tps_trans_defs) sorry
-  next
-    case (WCommit x1 x2 x3 x4 x5 x6 x7)
-    then show ?case apply (auto simp add: RO_has_rts_def tps_trans_defs split: if_split_asm) sorry
-    (* inv: if t : RO in K it remains RO in K' *)
-  qed (auto simp add: RO_has_rts_def tps_trans_defs)
-qed
-
-definition SO_ROs where
-  "SO_ROs s \<longleftrightarrow> (\<forall>r1 r2 rts1 rts2. (Tn r1, Tn r2) \<in> SO \<and>
-    rtxn_rts s r1 = Some rts1 \<and> rtxn_rts s r2 = Some rts2 \<longrightarrow> rts1 \<le> rts2)"
-
-lemmas SO_ROsI = SO_ROs_def[THEN iffD2, rule_format]
-lemmas SO_ROsE[elim] = SO_ROs_def[THEN iffD1, elim_format, rule_format]
-
-lemma reach_so_ro [simp]: "reach tps_s s \<Longrightarrow> SO_ROs s"
-proof(induction s rule: reach.induct)
-  case (reach_init s)
-  then show ?case by (auto simp add: SO_ROs_def tps_s_defs)
-next
-  case (reach_trans s e s')
-  then show ?case
-  proof (induction e)
-    case (RDone x1 x2 x3 x4 x5)
-    then show ?case apply (auto simp add: SO_ROs_def tps_trans_defs SO_def SO0_def)
-      apply (metis CFTid_Rtxn_Inv_def less_or_eq_imp_le option.distinct(1) reach_cftid_rtxn_inv)
-      by (meson Rtxn_rts_le_Gst_def reach_rtxn_rts_le_gst)
-  qed (auto simp add: SO_ROs_def tps_trans_defs)
-qed
-
-definition SO_RO_WR where
-  "SO_RO_WR s \<longleftrightarrow> (\<forall>r w rts cts. (Tn r, w) \<in> SO \<and>
-    rtxn_rts s r = Some rts \<and> wtxn_cts s w = Some cts \<longrightarrow> rts \<le> cts)"
-
-lemmas SO_RO_WRI = SO_RO_WR_def[THEN iffD2, rule_format]
-lemmas SO_RO_WRE[elim] = SO_RO_WR_def[THEN iffD1, elim_format, rule_format]
-
-lemma reach_so_ro_wr [simp]: "reach tps_s s \<Longrightarrow> SO_RO_WR s"
-proof(induction s rule: reach.induct)
-  case (reach_init s)
-  then show ?case by (auto simp add: SO_RO_WR_def tps_s_defs)
-next
-  case (reach_trans s e s')
-  then show ?case
-  proof (induction e)
-    case (WCommit x1 x2 x3 x4 x5 x6 x7)
-    then show ?case apply (auto simp add: SO_RO_WR_def tps_trans_defs SO_def SO0_def) sorry
-  next
-    case (RDone x1 x2 x3 x4 x5)
-    then show ?case apply (auto simp add: SO_RO_WR_def tps_trans_defs SO_def SO0_def) sorry
-  qed (auto simp add: SO_RO_WR_def tps_trans_defs)
-qed
-
-subsection \<open>Closedness\<close>
-lemma visTx'_union_distr: "visTx' K (u\<^sub>1 \<union> u\<^sub>2) = visTx' K u\<^sub>1 \<union> visTx' K u\<^sub>2"
-  by (auto simp add: visTx'_def)
-
-lemma visTx'_Union_distr: "visTx' K (\<Union>i\<in>I. u i) = (\<Union>i\<in>I. visTx' K (u i))"
-  by (auto simp add: visTx'_def)
-
-lemma visTx'_same_writers: "kvs_writers K' = kvs_writers K \<Longrightarrow> visTx' K' u = visTx' K u"
-  by (simp add: visTx'_def)
-
-lemma union_closed':
-  assumes "closed' K u\<^sub>1 r"
-    and "closed' K u\<^sub>2 r"
-    and "kvs_writers K' = kvs_writers K" 
-    and "read_only_Txs K \<subseteq> read_only_Txs K'"
-  shows "closed' K' (u\<^sub>1 \<union> u\<^sub>2) r"
+text \<open>View update lemmas\<close>
+
+lemma get_view_update_cls:
+  "cl' \<noteq> cl \<Longrightarrow>
+   get_view (s\<lparr>cls := (cls s)(cl := X) \<rparr>) cl' = get_view s cl'"
+  by (auto simp add: get_view_def)
+
+lemma get_view_update_cls_rtxn_rts:
+  "cl' \<noteq> cl \<Longrightarrow>
+   get_view (s\<lparr>cls := (cls s)(cl := X), rtxn_rts := Y \<rparr>) cl' = get_view s cl'"
+  by (auto simp add: get_view_def)
+
+lemma get_view_update_svr_wtxns_dom:
+   "wtxns_dom new_svr_state = wtxns_dom (svr_state (svrs s k)) \<Longrightarrow> 
+    get_view (s\<lparr>svrs := (svrs s)
+                   (k := svrs s k
+                      \<lparr>svr_state := new_svr_state,
+                       svr_clock := clk \<rparr>)\<rparr>) cl 
+ = get_view s cl"
+  by (auto simp add: get_view_def ext)
+
+
+lemma get_view_update_cls_wtxn_cts_cts_order:
+  "\<lbrakk> cl' \<noteq> cl; wtxn_cts s (get_wtxn s cl) = None; Y > gst (cls s cl') \<rbrakk> \<Longrightarrow>
+   get_view (s\<lparr> cls := (cls s)(cl := X),
+                wtxn_cts := (wtxn_cts s) (get_wtxn s cl \<mapsto> Y),
+                cts_order := Z \<rparr>) cl'
+  = get_view s cl'"
+  by (auto simp add: get_view_def)
+
+lemma get_view_update_svr_prep:
+  assumes "cl \<noteq> get_cl_w t"
+    "t \<noteq> T0"
+    "cl_state (cls s (get_cl_w t)) = WtxnPrep kv_map'"
+    "cl_sn (cls s (get_cl_w t)) = get_sn_w t"
+    "Wtxn_Cts_None s"
+  shows "get_view (s\<lparr>svrs := (svrs s)
+                   (k := svrs s k
+                      \<lparr>svr_state := (svr_state (svrs s k))(t := Prep pd ts v),
+                       svr_clock := clk \<rparr>)\<rparr>) cl 
+       = get_view s cl"
   using assms
-  by (auto simp add: closed'_def visTx'_union_distr visTx'_same_writers[of K']
-           intro: closed_general_set_union_closed)
-
-lemma Union_closed':
-  assumes "\<And>i. i \<in> I \<Longrightarrow> closed' K (u i) r"
-    and "finite I" 
-    and "kvs_writers K' = kvs_writers K" 
-    and "read_only_Txs K \<subseteq> read_only_Txs K'"
-  shows "closed' K' (\<Union>i\<in>I. u i) r"
-  using assms                                  
-  apply (simp add: closed'_def visTx'_Union_distr visTx'_same_writers[of K'])
-  apply (rule closed_general_set_Union_closed)
-  apply auto
-  done
-
-lemma union_closed'_extend_rel:
-  assumes "closed' K u\<^sub>1 r"
-    and "closed' K u\<^sub>2 r"
-    and "kvs_writers K' = kvs_writers K" 
-    and "read_only_Txs K \<subseteq> read_only_Txs K'"
-    and "x \<notin> (r\<inverse>)\<^sup>* `` (visTx' K u\<^sub>1 \<union> visTx' K u\<^sub>2)"
-    and "r' = (\<Union>y\<in>Y. {(y, x)}) \<union> r"
-    and "finite Y"
-  shows "closed' K' (u\<^sub>1 \<union> u\<^sub>2) r'"
-  using assms
-  by (auto simp add: closed'_def visTx'_union_distr visTx'_same_writers[of K']
-      intro: closed_general_union_V_extend_N_extend_rel)
-
-
-lemma visTx'_new_writer: "kvs_writers K' = insert t (kvs_writers K) \<Longrightarrow>
-  visTx' K' (insert t u) = insert t (visTx' K u)"
-  by (auto simp add: visTx'_def)
-
-lemma insert_wr_t_closed':
-  assumes "closed' K u r"
-    and "closed_general {t} (r\<inverse>) (visTx' K u \<union> read_only_Txs K)"
-    and "read_only_Txs K' = read_only_Txs K"
-    and "kvs_writers K' = insert t (kvs_writers K)"
-  shows "closed' K' (insert t u) r"
-  using assms
-  by (auto simp add: closed'_def visTx'_new_writer intro: closed_general_set_union_closed)
-
-\<comment> \<open>insert (k, t) in version's deps - used in get_ctx\<close>
-lemma visTx'_observes_t:
-  "t \<in> kvs_writers K \<Longrightarrow> visTx' K (insert t deps) = insert t (visTx' K deps)"
-  by (simp add: visTx'_def)
-
-lemma insert_kt_to_deps_closed':
-  assumes "closed' K deps r"
-    and "t \<in> kvs_writers K"
-    and "closed_general {t} (r\<inverse>) (visTx' K deps \<union> read_only_Txs K)"
-  shows "closed' K (insert t deps) r"
-  using assms
-  by (auto simp add: closed'_def visTx'_observes_t intro: closed_general_set_union_closed)
-
-(*
-\<comment> \<open>concrete read_done closedness\<close>
-
-\<comment> \<open>premises\<close>
-  
-lemma get_ctx_closed:
-  assumes "\<And>t. t \<in> read_wtxns s cl (dom kv_map) \<Longrightarrow>
-      closed' K (insert t (wtxn_deps s t)) r"
-    and "cl_state (cls s cl) = RtxnInProg (dom kv_map) kv_map"
-    and "Rtxn_RegK_Kvtm_Cmt_in_rs s cl"
-    and "Finite_Dom_Kv_map_rd s cl"
-  shows "closed' K (get_ctx s cl (dom kv_map)) r"
-  using assms
-  by (auto simp add: Finite_Dom_Kv_map_rd_def get_ctx_defs intro!: Union_closed')
-
-lemma v_writer_kvs_of_s:
-  assumes "\<forall>k. CO_not_No_Ver s k"
-  shows "v_writer ` (\<lambda>t. case svr_state (svrs s k) t of
-      Prep pd ts v \<Rightarrow> \<lparr>v_value = v, v_writer = t, v_readerset = {}\<rparr>
-    | Commit cts sts lst v rs \<Rightarrow> \<lparr>v_value = v, v_writer = t,
-        v_readerset = {t. \<exists>rts rlst. (t, rts, rlst) \<in> rs \<and> get_sn t < cl_sn (cls s (get_cl t))}\<rparr>) ` set (cts_order s k) =
-   {t \<in> set (cts_order s k). \<exists>pd ts v cts sts lst rs.
-        svr_state (svrs s k) t \<in> {Prep pd ts v, Commit cts sts lst v rs}}"
-  using assms
-  by (auto simp add: image_iff CO_not_No_Ver_def split: ver_state.split)
-
-lemma v_readerset_kvs_of_s_k:
-  assumes "\<forall>k. CO_not_No_Ver s k"
-    and "t_wr \<in> set (cts_order s k)"
-  shows "v_readerset (case svr_state (svrs s k) t_wr of
-      Prep pd ts v \<Rightarrow> \<lparr>v_value = v, v_writer = t_wr, v_readerset = {}\<rparr>
-    | Commit cts sts lst v rs \<Rightarrow> \<lparr>v_value = v, v_writer = t_wr,
-        v_readerset = {t. \<exists>rts rlst. (t, rts, rlst) \<in> rs \<and> get_sn t < cl_sn (cls s (get_cl t))}\<rparr>) = 
-   {t. \<exists>cts sts lst v rs rts rlst. svr_state (svrs s k) t_wr = Commit cts sts lst v rs \<and>
-      (t, rts, rlst) \<in> rs \<and> get_sn t < cl_sn (cls s (get_cl t))}"
-  using assms
-  by (auto split: ver_state.split)
-
-lemma v_readerset_kvs_of_s:
-  assumes "\<forall>k. CO_not_No_Ver s k"
-  shows "(\<Union>k. \<Union>t_wr\<in>set (cts_order s k). v_readerset (case svr_state (svrs s k) t_wr of
-      Prep pd ts v \<Rightarrow> \<lparr>v_value = v, v_writer = t_wr, v_readerset = {}\<rparr>
-    | Commit cts sts lst v rs \<Rightarrow> \<lparr>v_value = v, v_writer = t_wr,
-        v_readerset = {t. \<exists>rts rlst. (t, rts, rlst) \<in> rs \<and> get_sn t < cl_sn (cls s (get_cl t))}\<rparr>)) = 
-   {t. \<exists>k. \<exists>t_wr \<in> set (cts_order s k).
-      \<exists>cts sts lst v rs rts rlst. svr_state (svrs s k) t_wr = Commit cts sts lst v rs \<and>
-      (t, rts, rlst) \<in> rs \<and> get_sn t < cl_sn (cls s (get_cl t))}"
-  using assms
-  apply (auto simp add: v_readerset_kvs_of_s_k)
-  by blast+
-
-lemma read_done_same_writers:
-  assumes "read_done cl kv_map sn u'' s s'"
-    and "\<forall>k. CO_not_No_Ver s k"
-    and "\<forall>k. CO_not_No_Ver s' k"
-  shows "kvs_writers (kvs_of_s s') = kvs_writers (kvs_of_s s)"
-  using assms
-  apply (simp add: kvs_writers_def vl_writers_def kvs_of_s_defs v_writer_kvs_of_s CO_not_No_Ver_def)
-  by (simp add: read_done_def read_done_U_def)
-
-lemma insert_Diff_if': "a \<notin> c \<Longrightarrow> insert a (b - c) = insert a b - c"
-  by (simp add: insert_Diff_if)
-
-lemma read_done_new_read:
-  assumes "read_done cl kv_map sn u'' s s'"
-    and "\<forall>k. CO_not_No_Ver s k"
-    and "\<forall>k. CO_not_No_Ver s' k"
-    and "\<forall>k. Committed_Abs_in_CO s k"
-    and "\<forall>k. T0_in_CO s k"
-    and "Finite_Dom_Kv_map_rd s cl"
-    and "Rtxn_RegK_Kvtm_Cmt_in_rs s cl"
-    and "Rtxn_RegK_Kvtm_Cmt_in_rs s cl"
-    and "Tn (get_txn s cl) \<notin> kvs_writers (kvs_of_s s)"
-  shows "read_only_Txs (kvs_of_s s') = insert (Tn (get_txn s cl)) (read_only_Txs (kvs_of_s s))"
-  using assms
-  apply (simp add: read_only_Txs_def read_done_same_writers insert_Diff_if')
-  apply (rule arg_cong[where f="\<lambda>m. m - _"])
-  apply (simp add: kvs_readers_def vl_readers_def kvs_of_s_defs v_readerset_kvs_of_s)
-  apply (auto simp add: tps_trans_defs image_insert[symmetric] simp del: image_insert)
-  using image_eqI apply blast
-  apply (smt (z3) image_eqI insertCI less_SucE mem_Collect_eq txid0.collapse)
-  using image_eqI apply blast
-  subgoal apply (rule image_eqI, auto)
-    apply (cases "dom kv_map = {}", auto simp add: ex_in_conv[symmetric] simp del: dom_eq_empty_conv)
-    subgoal for k v apply (rule exI[where x=k])
-      by (metis (lifting) Rtxn_RegK_Kvtm_Cmt_in_rs_def Committed_Abs_in_CO_def)
-    done
-  by (smt (verit) image_eqI less_Suc_eq mem_Collect_eq)
-
-lemma fresh_rtxn_not_vis:
-  assumes "Tn (get_txn s cl) \<notin> kvs_writers (kvs_of_s s)"
-    and "\<forall>t \<in> kvs_writers (kvs_of_s s). get_sn_w t < cl_sn (cls s cl)"
-  shows "Tn (get_txn s cl) \<notin> ((R_CC (kvs_of_s s))\<inverse>)\<^sup>* `` (visTx' (kvs_of_s s)
-    (cl_ctx (cls s cl) \<union> get_ctx s cl keys))"
-  apply (auto simp add: visTx'_def R_CC_def)
-  subgoal for t apply (induction t "Tn (get_txn s cl)" rule: rtrancl.induct, auto)
-      apply (simp add: assms(1))
-     apply (simp add: SO_def SO0_def) oops
-
-lemma read_done_WR_onK:
-  assumes "read_done cl kv_map sn u'' s s'"
-  shows "R_onK WR (kvs_of_s s') = (read_wtxns s cl (dom kv_map) \<times> {Tn (get_txn s cl)}) \<union> R_onK WR (kvs_of_s s)"
-  apply (auto simp add: R_onK_def WR_def) sorry
-
-lemma read_done_extend_rel:
-  assumes "read_done cl kv_map sn u'' s s'"
-  shows "R_CC (kvs_of_s s') = (read_wtxns s cl (dom kv_map) \<times> {Tn (get_txn s cl)}) \<union> R_CC (kvs_of_s s)"
-  using assms
-  by (auto simp add: R_CC_def read_done_WR_onK)
-
-
-\<comment> \<open>read_done closedness (canCommit)\<close>
-lemma read_done_ctx_closed:
-  assumes "closed' (kvs_of_s s) (cl_ctx (cls s cl)) (R_CC (kvs_of_s s))"
-    and "closed' (kvs_of_s s) (get_ctx s cl keys) (R_CC (kvs_of_s s))"
-    and "kvs_writers (kvs_of_s s') = kvs_writers (kvs_of_s s)"
-    and "read_only_Txs (kvs_of_s s') = insert (Tn (get_txn s cl)) (read_only_Txs (kvs_of_s s))"
-    and "Tn (get_txn s cl) \<notin> ((R_CC (kvs_of_s s))\<inverse>)\<^sup>* ``
-      (visTx' (kvs_of_s s) (cl_ctx (cls s cl) \<union> get_ctx s cl keys))"
-    and "R_CC (kvs_of_s s') = (read_wtxns s cl keys \<times> {Tn (get_txn s cl)}) \<union> R_CC (kvs_of_s s)"
-    and "Finite_Keys s cl"
-    and "cl_state (cls s cl) = RtxnInProg cclk keys kv_map"
-  shows "closed' (kvs_of_s s') (cl_ctx (cls s cl) \<union> get_ctx s cl keys) (R_CC (kvs_of_s s'))"
-  using assms
-  by (auto simp add: closed'_def visTx'_union_distr visTx'_same_writers[of "kvs_of_s s'"] finite_read_wtxns
-    Finite_Keys_def intro: closed_general_union_V_extend_N_extend_rel[where Y="read_wtxns s cl keys"]) old lemmas*)
-                                                            
-\<comment> \<open>write_commit closedness (canCommit)\<close>
-lemma write_commit_WR_onK:
-  assumes "write_commit cl kv_map commit_t sn u'' clk mmap s s'"
-  shows "R_onK WR (kvs_of_s s') = R_onK WR (kvs_of_s s)"
-  apply (auto simp add: R_onK_def WR_def) sorry
-
-lemma write_commit_same_rel:
-  assumes "write_commit cl kv_map commit_t sn u'' clk mmap s s'"
-  shows "R_CC (kvs_of_s s') = R_CC (kvs_of_s s)"
-  using assms
-  by (auto simp add: R_CC_def write_commit_WR_onK)
-
-lemma "dom kv_map \<noteq> {} \<Longrightarrow> snd ` (\<Union>k\<in>dom kv_map. {(k, t)}) = {t}"
-  apply (auto simp add: image_def)
-  by (metis domIff insertI1 sndI)
-
-lemma write_commit_ctx_closed:    (* HERE *)
-  assumes "write_commit cl kv_map commit_t sn u'' clk mmap s s'"
-    and "closed' (kvs_of_s s) (cl_ctx (cls s cl)) (R_CC (kvs_of_s s))"
-    and "closed_general {get_wtxn s cl} ((R_CC (kvs_of_s s))\<inverse>)
-          (visTx' (kvs_of_s s) (cl_ctx (cls s cl)) \<union> read_only_Txs (kvs_of_s s))"
-    and "read_only_Txs (kvs_of_s s') = read_only_Txs (kvs_of_s s)"
-    and "kvs_writers (kvs_of_s s') = insert (get_wtxn s cl) (kvs_writers (kvs_of_s s))"
-  shows "closed' (kvs_of_s s') (insert (get_wtxn s cl) (cl_ctx (cls s cl))) (R_CC (kvs_of_s s'))"
-  using assms
-  apply (auto simp add: closed'_def write_commit_same_rel image_def intro: insert_wr_t_closed') 
-  sorry
-
-
-subsection \<open>CanCommit\<close>
-
-lemma the_T0: "(THE i. i = 0 \<and> [T0] ! i = T0) = 0" by auto
-
-lemmas canCommit_defs = ET_CC.canCommit_def R_CC_def R_onK_def
-
-(*lemma visTx_visTx': "\<comment> \<open>\<forall>k t. (k, t) \<in> u \<longrightarrow> t \<in> set (cts_order s k) \<Longrightarrow>\<close>
-  visTx (kvs_of_s s) (view_of (cts_order s) u) = visTx' (kvs_of_s s) u"
-  apply (auto simp add: visTx_def visTx'_def (* kvs_writers_def vl_writers_def image_iff*) ) 
-  
-  sorry
-
-lemma closed_closed': "closed (kvs_of_s s) (view_of (cts_order s) u) r = closed' (kvs_of_s s) u r"
-  by (simp add: closed'_def visTx_visTx') *)
-
-lemma visTx'_cl_ctx_subset_writers:
-  "visTx' (kvs_of_s s) (cl_ctx (cls s cl)) \<subseteq> kvs_writers (kvs_of_s s)"
-  by (simp add: visTx'_def)
-
-lemma visTx'_wtxn_deps_subset_writers: 
-  "wtxn_deps s t = deps \<Longrightarrow> visTx' (kvs_of_s s) deps \<subseteq> kvs_writers (kvs_of_s s)"
-  by (simp add: visTx'_def)
-
-lemma "kvs_writers (kvs_of_s s) \<subseteq> (\<Union>k. wtxns_dom (svr_state (svrs s k)))"
-  oops
-
-lemma "kvs_readers (kvs_of_s s) \<subseteq> (\<Union>k. wtxns_rsran (svr_state (svrs s k)))"
-  oops
-
-definition RO_le_gst :: "'v global_conf \<Rightarrow> cl_id \<Rightarrow> txid set" where
-  "RO_le_gst s cl \<equiv> {t \<in> read_only_Txs (kvs_of_s s). \<exists>t'. t = Tn t' \<and> the (rtxn_rts s t') \<le> gst (cls s cl)}"
-
-definition RO_WO_Inv where
-  "RO_WO_Inv s \<longleftrightarrow> (\<Union>k. wtxns_dom (svr_state (svrs s k))) \<inter> Tn ` (\<Union>k. wtxns_rsran (svr_state (svrs s k))) = {}"
-
-lemmas RO_WO_InvI = RO_WO_Inv_def[THEN iffD2, rule_format]
-lemmas RO_WO_InvE[elim] = RO_WO_Inv_def[THEN iffD1, elim_format, rule_format]
-
-lemma reach_ro_wo_inv [simp]: "reach tps_s s \<Longrightarrow> RO_WO_Inv s"
-proof(induction s rule: reach.induct)
-  case (reach_init s)
-  then show ?case
-    by (auto simp add: RO_WO_Inv_def tps_s_defs)
-next
-  case (reach_trans s e s')
-  then show ?case 
-  proof (induction e)
-    case (RegR x1 x2 x3 x4 x5 x6 x7)
-    then show ?case apply (auto simp add: RO_WO_Inv_def tps_trans_defs) sorry
-     (*using add_to_readerset_v_writer_img[of ] apply (simp add: txid_defs) sorry \<comment> \<open>Continue here!\<close>*)
-  next
-    case (PrepW x1 x2 x3 x4 x5)
-    then show ?case sorry
-  next
-    case (CommitW x1 x2 x3 x4 x5 x6 x7)
-    then show ?case sorry
-  qed (auto simp add: RO_WO_Inv_def tps_trans_defs)
-qed
-
-
-subsection \<open>View Invariants\<close>
-
-definition View_Init where
-  "View_Init s cl k \<longleftrightarrow> (T0 \<in> get_view s cl k)"
-
-lemmas View_InitI = View_Init_def[THEN iffD2, rule_format]
-lemmas View_InitE[elim] = View_Init_def[THEN iffD1, elim_format, rule_format]
-
-lemma reach_view_init [simp]: "reach tps_s s \<Longrightarrow> View_Init s cl k"
-proof(induction s rule: reach.induct)
-  case (reach_init s)
-  then show ?case
-    by (auto simp add: View_Init_def tps_s_defs get_view_def)
-next
-  case (reach_trans s e s')
-  then show ?case 
-  proof (induction e)
-    case (RInvoke x1 x2 x3 x4)
-    then show ?case apply (simp add: View_Init_def tps_trans_defs get_view_def)
-      by (meson Gst_le_Min_Lst_map_def linorder_not_le order.strict_trans2
-          reach_gst_le_min_lst_map reach_gst_lt_cl_cts)
-  next
-    case (RegR x1 x2 x3 x4 x5 x6 x7)
-    then show ?case apply (simp add: View_Init_def tps_trans_defs get_view_def)
-      using add_to_readerset_no_ver_inv by blast
-  qed (auto simp add: View_Init_def tps_trans_defs get_view_def)
-qed
-
-
-definition Get_View_Committed where
-  "Get_View_Committed s cl k \<longleftrightarrow> (\<forall>t. t \<in> get_view s cl k  \<longrightarrow>
-    (is_committed (svr_state (svrs s k) t) \<or> 
-    (\<exists>cts kv_map. cl_state (cls s cl) = WtxnCommit cts kv_map \<and> k \<in> dom kv_map \<and> t = get_wtxn s cl)))"
-
-lemmas Get_View_CommittedI = Get_View_Committed_def[THEN iffD2, rule_format]
-lemmas Get_View_CommittedE[elim] = Get_View_Committed_def[THEN iffD1, elim_format, rule_format]
-
-lemma reach_get_view_committed[simp]:
-  "reach tps_s s \<Longrightarrow> Get_View_Committed s cl k"
-proof(induction s rule: reach.induct)
-  case (reach_init s)
-  then show ?case by (auto simp add: Get_View_Committed_def tps_s_defs get_view_def)
-next
-  case (reach_trans s e s')
-  then show ?case
-  proof (induction e)
-    case (RInvoke x1 x2 x3 x4)
-    then show ?case apply (auto simp add: Get_View_Committed_def tps_trans_defs get_view_def) sorry
-  next
-    case (WCommit x1 x2 x3 x4 x5 x6 x7)
-    then show ?case apply (auto simp add: Get_View_Committed_def tps_trans_defs get_view_def) sorry
-  next
-    case (WDone x1 x2 x3 x4 x5)
-    then show ?case apply (auto simp add: Get_View_Committed_def tps_trans_defs get_view_def) sorry
-  next
-    case (RegR x1 x2 x3 x4 x5 x6 x7)
-    then show ?case apply (auto simp add: Get_View_Committed_def tps_trans_defs get_view_def) sorry
-  next
-    case (PrepW x1 x2 x3 x4 x5)
-    then show ?case apply (auto simp add: Get_View_Committed_def tps_trans_defs get_view_def) sorry
-  qed (auto simp add: Get_View_Committed_def tps_trans_defs get_view_def)
-qed
-
-(* Closedness inv
-definition Deps_Closed where
-  "Deps_Closed s cl \<longleftrightarrow> (closed' (kvs_of_s s) (get_view s cl) (R_CC (kvs_of_s s)) \<and> 
-    (\<forall>k t cts sts lst v rs kv_map deps. svr_state (svrs s k) t = Commit cts sts lst v rs \<or>
-      cl_state (cls s cl) = WtxnCommit cts kv_map \<longrightarrow>
-      closed' (kvs_of_s s) deps (R_CC (kvs_of_s s))))"
-
-lemmas Deps_ClosedI = Deps_Closed_def[THEN iffD2, rule_format]
-lemmas Deps_ClosedE[elim] = Deps_Closed_def[THEN iffD1, elim_format, rule_format]
-
-lemmas closed'_defs = closed'_def R_CC_def R_onK_def
-
-lemma reach_deps_closed[simp]:
-  "reach tps_s s \<Longrightarrow> Deps_Closed s cl"
-proof(induction s rule: reach.induct)
-  case (reach_init s)
-  then show ?case apply (auto simp add: Deps_Closed_def tps_def) sorry
-next
-  case (reach_trans s e s')
-  then show ?case using kvs_of_s_inv[of s e s']
-  proof (induction e)
-    case (RDone x1 x2 x3 x4 x5)
-    then show ?case using read_done_ctx_closed get_ctx_closed
-      apply (auto simp add: Deps_Closed_def tps_trans_defs) sorry
-  next
-    case (WCommit x1 x2 x3 x4 x5 x6 x7)
-    then show ?case apply (simp add: Deps_Closed_def tps_trans_defs) sorry
-  next
-    case (RegR x1 x2 x3 x4 x5 x6 x7)
-    then show ?case sorry
-  next
-    case (CommitW x1 x2 x3 x4 x5 x6 x7)
-    then show ?case sorry
-  qed (auto simp add: Deps_Closed_def tps_trans_defs)
-qed
-*)
-
-
-subsection \<open>View Shift\<close>
-
-definition Cl_WtxnCommit_Get_View where
-  "Cl_WtxnCommit_Get_View s cl \<longleftrightarrow>
-    (\<forall>cts kv_map. cl_state (cls s cl) = WtxnCommit cts kv_map \<longrightarrow>
-      (\<forall>k \<in> dom kv_map. get_wtxn s cl \<in> get_view s cl k))"
-
-lemmas Cl_WtxnCommit_Get_ViewI = Cl_WtxnCommit_Get_View_def[THEN iffD2, rule_format]
-lemmas Cl_WtxnCommit_Get_ViewE[elim] = Cl_WtxnCommit_Get_View_def[THEN iffD1, elim_format, rule_format]
-
-lemma reach_cl_wtxncommit_get_view [simp]: "reach tps_s s \<Longrightarrow> Cl_WtxnCommit_Get_View s cl"
-proof(induction s rule: reach.induct)
-  case (reach_init s)
-  then show ?case
-    by (auto simp add: Cl_WtxnCommit_Get_View_def tps_s_defs)
-next
-  case (reach_trans s e s')
-  then show ?case
-  proof (induction e)
-    case (WCommit x1 x2 x3 x4 x5 x6 x7)
-    then show ?case apply (simp add: Cl_WtxnCommit_Get_View_def tps_trans_defs get_view_def)
-      by (meson domI wtxns_domI1 wtxns_domIff)
-  next
-    case (RegR x1 x2 x3 x4 x5 x6 x7)
-    then show ?case apply (simp add: Cl_WtxnCommit_Get_View_def tps_trans_defs get_view_def)
-      by (simp add: add_to_readerset_wtxns_dom)
-  qed (auto simp add: Cl_WtxnCommit_Get_View_def tps_trans_defs get_view_def)
-qed
-
-lemma read_commit_added_txid:
-  assumes "read_done cl kv_map sn u clk s s'"
-    and "Tn (Tn_cl sn' cl) \<in> (kvs_txids (kvs_of_s s') - kvs_txids (kvs_of_s s))"
-  shows "sn' = sn"
-  using assms
-  apply (auto simp add: read_done_def kvs_of_s_defs txid_defs split: ver_state.split) sorry
-
-subsection \<open>Fp Property\<close>
-
-\<comment> \<open>Fingerprint content invariant and Lemmas for proving the fp_property\<close>
-
-definition RegR_Fp_Inv where
-  "RegR_Fp_Inv s k \<longleftrightarrow> (\<forall>t cclk keys kv_map cts sts lst v rs.
-    cl_state (cls s (get_cl t)) = RtxnInProg cclk keys kv_map \<and> k \<in> keys \<and> kv_map k = None \<and>
-    svr_state (svrs s k) (read_at (svr_state (svrs s k)) (gst (cls s (get_cl t))) (get_cl t))
-       = Commit cts sts lst v rs \<longrightarrow>
-    v = v_value ((kvs_of_s s k) !
-      Max (view_of (cts_order s) (get_view s (get_cl t)) k)))"
-
-lemmas RegR_Fp_InvI = RegR_Fp_Inv_def[THEN iffD2, rule_format]
-lemmas RegR_Fp_InvE[elim] = RegR_Fp_Inv_def[THEN iffD1, elim_format, rule_format]
-
-lemma reach_reg_r_fp [simp]: "reach tps_s s \<Longrightarrow> RegR_Fp_Inv s cl"
-proof(induction s rule: reach.induct)
-  case (reach_init s)
-  then show ?case by (auto simp add: RegR_Fp_Inv_def tps_s_defs)
-next
-  case (reach_trans s e s')
-  then show ?case using kvs_of_s_inv[of s e s']
-  proof (induction e)
-    case (RInvoke x1 x2 x3 x4)
-    then show ?case apply (auto simp add: RegR_Fp_Inv_def tps_trans_defs) sorry
-  next
-    case (Read x1 x2 x3 x4 x5 x6 x7)
-    then show ?case apply (auto simp add: RegR_Fp_Inv_def tps_trans_defs) sorry
-  next
-    case (RDone x1 x2 x3 x4 x5)
-    then show ?case apply (auto simp add: RegR_Fp_Inv_def tps_trans_defs) sorry
-  next
-    case (WCommit x1 x2 x3 x4 x5 x6 x7)
-    then show ?case apply (auto simp add: RegR_Fp_Inv_def tps_trans_defs) sorry
-  next
-    case (RegR x1 x2 x3 x4 x5 x6 x7)
-    then show ?case apply (auto simp add: RegR_Fp_Inv_def tps_trans_defs) sorry
-  next
-    case (PrepW x1 x2 x3 x4 x5)
-    then show ?case apply (auto simp add: RegR_Fp_Inv_def tps_trans_defs) sorry
-  next
-    case (CommitW x1 x2 x3 x4 x5 x6 x7)
-    then show ?case apply (auto simp add: RegR_Fp_Inv_def tps_trans_defs) sorry
-  qed (auto simp add: RegR_Fp_Inv_def tps_trans_defs get_view_def)
-qed
-
-(* more inv to show v_value v_writer kvs_of_s commit_t kv_map relation*)
-
-definition Rtxn_Fp_Inv where
-  "Rtxn_Fp_Inv s cl \<longleftrightarrow> (\<forall>k cclk keys kv_map v.
-    cl_state (cls s cl) = RtxnInProg cclk keys kv_map \<and> kv_map k = Some v \<longrightarrow>
-     v = v_value ((kvs_of_s s k) !
-        Max (view_of (cts_order s) (get_view s cl) k)))"
-
-lemmas Rtxn_Fp_InvI = Rtxn_Fp_Inv_def[THEN iffD2, rule_format]
-lemmas Rtxn_Fp_InvE[elim] = Rtxn_Fp_Inv_def[THEN iffD1, elim_format, rule_format]
-
-lemma reach_rtxn_fp [simp]: "reach tps_s s \<Longrightarrow> Rtxn_Fp_Inv s cl"
-proof(induction s rule: reach.induct)
-  case (reach_init s)
-  then show ?case by (auto simp add: Rtxn_Fp_Inv_def tps_s_defs)
-next
-  case (reach_trans s e s')
-  then show ?case using kvs_of_s_inv[of s e s']
-  proof (induction e)
-    case (Read x1 x2 x3 x4 x5 x6 x7)
-    then show ?case apply (auto simp add: Rtxn_Fp_Inv_def tps_trans_defs) sorry
-  next
-    case (RDone x1 x2 x3 x4 x5)
-    then show ?case sorry
-  next
-    case (WCommit x1 x2 x3 x4 x5 x6 x7)
-    then show ?case sorry
-  next
-    case (RegR x1 x2 x3 x4 x5 x6 x7)
-    then show ?case sorry
-  next
-    case (PrepW x1 x2 x3 x4 x5)
-    then show ?case sorry
-  next
-    case (CommitW x1 x2 x3 x4 x5 x6 x7)
-    then show ?case sorry
-  qed (auto simp add: Rtxn_Fp_Inv_def tps_trans_defs view_of_def get_view_def)
-qed
-
-definition Rtxn_notin_rs_other_t where
-  "Rtxn_notin_rs_other_t s cl \<longleftrightarrow>
-   (\<forall>k cclk keys kv_map t cts sts lst v rs t' cts' sts' lst' v' rs' rts rlst.
-    cl_state (cls s cl) = RtxnInProg cclk keys kv_map \<and>
-    svr_state (svrs s k) t = Commit cts sts lst v rs \<and> rs (get_txn s cl) = Some (rts, rlst) \<and>
-    \<comment> \<open>try: t' \<noteq> cts_order s k ! Max (view_of (cts_order s) (cl_ctx (cls s cl) \<union> get_ctx s cl keys) k) \<and>\<close>
-    svr_state (svrs s k) t' = Commit cts' sts' lst' v' rs' \<longrightarrow> rs' (get_txn s cl) = None)"
-
-lemmas Rtxn_notin_rs_other_tI = Rtxn_notin_rs_other_t_def[THEN iffD2, rule_format]
-lemmas Rtxn_notin_rs_other_tE[elim] = Rtxn_notin_rs_other_t_def[THEN iffD1, elim_format, rule_format]
-
-lemma reach_rtxn_notin_rs_other_t [simp]: "reach tps_s s \<Longrightarrow> Rtxn_notin_rs_other_t s cl"
-proof(induction s rule: reach.induct)
-  case (reach_init s)
-  then show ?case by (auto simp add: Rtxn_notin_rs_other_t_def tps_s_defs)
-next
-  case (reach_trans s e s')
-  then show ?case 
-  proof (induction e)
-    case (RInvoke x1 x2 x3 x4)
-    then show ?case sorry
-next
-    case (Read x1 x2 x3 x4 x5 x6 x7)
-    then show ?case apply (auto simp add: Rtxn_notin_rs_other_t_def tps_trans_defs)
-      by meson
-  next
-    case (RegR x1 x2 x3 x4 x5 x6 x7)
-    then show ?case apply (auto simp add: Rtxn_notin_rs_other_t_def tps_trans_defs
-          split: ver_state.split) sorry
-  next
-    case (PrepW x1 x2 x3 x4 x5)
-    then show ?case by (simp add: Rtxn_notin_rs_other_t_def tps_trans_defs, blast)
-  next
-    case (CommitW x1 x2 x3 x4 x5 x6 x7)
-    then show ?case by (simp add: Rtxn_notin_rs_other_t_def tps_trans_defs, blast)
-  qed (auto simp add: Rtxn_notin_rs_other_t_def tps_trans_defs)
-qed
-
-
-subsection \<open>Proofs in progress\<close>
-
-(**************************************)
-(**************************************)
-
-(* lemmas about lists *)
-
-(*
-lemma 
-  "\<lbrakk> distinct xs; x \<in> set xs \<rbrakk> \<Longrightarrow> \<exists>!i. i < length xs \<and> xs ! i = x"
-  by (fact distinct_Ex1)
-*)
-
-lemma distinct_prefix:
-  "\<lbrakk> distinct xs; prefix xs' xs \<rbrakk> \<Longrightarrow> distinct xs'"
-  by (metis distinct_append prefixE)
-
-lemma nth_eq_prefix:
-  "\<lbrakk> i < length xs; prefix xs ys \<rbrakk> \<Longrightarrow> xs ! i = ys ! i"
-  by (metis nth_append prefix_def)
-
-
-lemma nth_distinct_injective:
-  "\<lbrakk> xs ! i = xs ! j; i < length xs; j < length xs; distinct xs \<rbrakk> \<Longrightarrow> i = j"
-  using nth_eq_iff_index_eq by blast
-
-
-(* lemma about THE *)
-
-lemma the_the_equality:
-  "\<lbrakk> P a; \<And>y. P y \<Longrightarrow> y = a; \<And>x. Q x \<longleftrightarrow> P x \<rbrakk> \<Longrightarrow> (THE x. P x) = (THE x. Q x)"
-  by (rule theI2) auto
-
-
-
-
-(* write_commit: preservation lemmas *)
-
-thm kvs_of_s_defs
-
-(*
-lemma write_commit_cl_sn_update:
-  assumes 
-    "write_commit cl kv_map cts sn u'' gs gs'"
-  shows
-    "cl_sn (cls gs' cl') = cl_sn (cls gs cl')"
-  using assms
-  by (auto simp add: write_commit_def) 
-*)
-
-
-(* 
-  lemmas about views 
-*)
-
-lemma get_view_cls_update:
- "\<forall>k\<in>dom kv_map. \<forall>t\<in>set (cts_order gs k). unique_ts (wtxn_cts gs) t < (cts, cl) \<Longrightarrow>
-   cts > gst (cls gs cl') \<Longrightarrow>
-    get_view (gs\<lparr>cls := (cls gs)(cl := cls gs cl\<lparr>cl_state := X, cl_clock := Y\<rparr>),
-                  wtxn_cts := (wtxn_cts gs)(get_wtxn gs cl \<mapsto> cts),
-                  cts_order := new_cord \<rparr>) cl'
-  = get_view gs cl'"
-  apply (auto simp add: get_view_def; rule ext, auto) oops
-
-lemma views_of_s_cls_update:  (* STILL NEEDED? *)
-  "\<forall>k\<in>dom kv_map. \<forall>t\<in>set (cts_order gs k). unique_ts (wtxn_cts gs) t < (cts, cl) \<Longrightarrow>
-   views_of_s (gs\<lparr>cls := (cls gs)(cl := cls gs cl\<lparr>cl_state := X, cl_clock := Y\<rparr>),
-                  wtxn_cts := (wtxn_cts gs)(get_wtxn gs cl \<mapsto> cts),
-                  cts_order := new_cord \<rparr>) cl' = 
-   view_of new_cord (get_view gs cl')"
-  apply (auto simp add: views_of_s_def get_view_def)
-  subgoal apply (intro arg_cong[where f="view_of new_cord"] ext)
-    apply auto sorry
-  subgoal apply (intro arg_cong[where f="view_of new_cord"] ext)
-    apply auto
-    subgoal sorry
-    subgoal sorry
-    subgoal sorry
-    oops
-
-thm view_of_def
-term view_of
-
-
-lemma view_of_deps_mono:     (* same as view_grows_view_of *)
-  assumes "\<forall>k. u k \<subseteq> u' k"
-  shows "view_of cord u \<sqsubseteq> view_of cord u'"
-  using assms
-  by (auto simp add: view_of_def view_order_def)
-
-text \<open>Note: we must have @{prop "distinct corder"} for @{term view_of} to be well-defined. \<close>
-
-
-thm ex1E
-thm the1_equality the1_equality' the_equality theI theI2
-thm prefix_length_le nth_eq_iff_index_eq
-
-lemma view_of_mono: 
-  assumes "\<forall>k. u k \<subseteq> u' k" and "\<And>k. prefix (cord k) (cord' k)" "\<And>k. distinct (cord' k)" 
-  shows "view_of cord u \<sqsubseteq> view_of cord' u'"
-  using assms
-proof -
-  { 
-    fix k t i
-    assume "t \<in> set (cord k)" 
-    have "distinct (cord' k)" "distinct (cord k)" 
-      using assms(2-3) by (auto dest: distinct_prefix) 
-    have "prefix (cord k) (cord' k)" "set (cord k) \<subseteq> set (cord' k)" "length (cord k) \<le> length (cord' k)"
-      using assms(2) by (auto dest: set_mono_prefix prefix_length_le)
-    then have "\<exists>!i. i < length (cord k) \<and> cord k ! i = t"  
-      using \<open>distinct (cord k)\<close> \<open>t \<in> set (cord k)\<close> by (intro distinct_Ex1) auto
-    then obtain i where
-      Pi: "i < length (cord k)" "cord k ! i = t" and
-      Pj: "\<And>j. \<lbrakk> j < length (cord k); cord k ! j = t \<rbrakk> \<Longrightarrow> j = i"
-      by (elim ex1E) auto
-    have "index_of (cord k) t = index_of (cord' k) t" 
-      using \<open>prefix (cord k) (cord' k)\<close> \<open>distinct (cord k)\<close> \<open>distinct (cord' k)\<close> 
-            \<open>length (cord k) \<le> length (cord' k)\<close> Pi
-      by (auto simp add: nth_eq_prefix nth_eq_iff_index_eq  intro: the_the_equality)
-  }
-  then show ?thesis using assms 
-    by (fastforce simp add: view_of_def view_order_def dest: set_mono_prefix)
-qed
-(*
-
-lemma view_of_ext_corder_cl_ctx:  
-  assumes "\<And>k. distinct (ext_corder (get_wtxn gs cl) kv_map (cts_order gs) k)"
-  shows "view_of (cts_order gs) (cl_ctx (cls gs cl)) \<sqsubseteq> 
-         view_of (ext_corder (get_wtxn gs cl) kv_map (cts_order gs)) 
-                 (insert (get_wtxn gs cl) (cl_ctx (cls gs cl)))"
-  using assms
-  by (intro view_of_mono) (auto simp add: ext_corder_def)
-
-*)
-
-(*
-  lemmas about KVS updates
-*)
-
-
-lemma update_kv_new_txid__DO_NOT_USE:   
-  assumes 
-    "t \<in> kvs_txids (update_kv t0 (write_only_fp kv_map) u K)" 
-    "t \<notin> kvs_txids K"
-  shows
-    "t = Tn t0"
-  using assms
-  by (simp add: kvs_txids_update_kv_write_only split: if_split_asm)
-
-
-
-(************)
-
-(*
-  more lemmas about view updates
-
-lemma view_of_update:
-  assumes 
-    "i = length (cord k)"  
-    "cord' k = cord k @ [t]"
-    "t \<notin> set (cord k)"
-    "t \<in> deps"
-  shows "i \<in> view_of cord' deps k"
-  using assms
-  apply (auto simp add: view_of_def)
-  apply (rule exI[where x=t])
-  apply (auto simp add: nth_append in_set_conv_nth intro: the_equality[symmetric] 
-              split: if_split_asm)
-  done
-
-
-
-lemma DO_NOT_USE_THIS: 
-  assumes 
-    "i < Suc (length (kvs_of_s gs k))"  
-    "\<not> i < length (kvs_of_s gs k)"
-    "get_wtxn gs cl \<notin> kvs_txids (kvs_of_s gs)"
-    "kv_map k = Some v" 
-    (* following two must be derived from invariants *)
-    "length (kvs_of_s gs k) = length (cts_order gs k)"
-    "get_wtxn gs cl \<notin> set (cts_order gs k)"
-  shows 
-  "i \<in> view_of (ext_corder (get_wtxn gs cl) kv_map (cts_order gs)) 
-               (insert (get_wtxn gs cl) (cl_ctx (cls gs cl))) k"
-  using assms 
-  by (intro view_of_update) (auto simp add: ext_corder_def)
-
-
-lemma view_of_update2:
-  assumes 
-    "i = length (cord k)"  
-    "cord' k = cord k @ [t]"
-    "t \<in> deps"
-    "(t, t') \<in> SO"
-    "t' \<notin> set (cord k)"
-  shows 
-    "i \<in> view_of cord' deps k"
-  apply (auto simp add: view_of_def)
-  apply (rule exI[where x=t])
-  apply (auto simp add: nth_append in_set_conv_nth intro!: the_equality[symmetric] 
-              split: if_split_asm)
-  oops
-
-
-lemma IS_THIS_USEFUL_QM:
-  "\<lbrakk>kv_map k = None; i < length (corder k); distinct (corder k); corder k ! i \<in> clctx\<rbrakk>
- \<Longrightarrow> i \<in> view_of (ext_corder t kv_map corder) 
-                 (insert (get_wtxn gs cl) clctx) k"
-  apply (auto simp add: view_of_def ext_corder_def)
-  apply (rule exI[where x="corder k ! i"])
-  apply auto
-  apply (rule the_equality[symmetric], auto dest: nth_distinct_injective)
-  done*)
-
-
-(************)
-
-(*
-  lemmas related to commit order (CO)
-*)
-
-lemma length_cts_order: "length (cts_order gs k) = length (kvs_of_s gs k)" 
-  by (simp add: kvs_of_s_def)
-
-lemma v_writer_txn_to_vers_inverse_on_CO:
-  assumes "CO_not_No_Ver gs k" "t \<in> set (cts_order gs k)"
-  shows "v_writer (txn_to_vers gs k t) = t"
-  using assms
-  by (auto simp add: txn_to_vers_def split: ver_state.split)
-
-
-lemma set_cts_order_incl_kvs_writers:
-  assumes "CO_not_No_Ver gs k"
-  shows "set (cts_order gs k) \<subseteq> kvs_writers (kvs_of_s gs)"
-  using assms
-  by (auto simp add: kvs_writers_def vl_writers_def kvs_of_s_def 
-                     v_writer_txn_to_vers_inverse_on_CO image_image
-           intro!: exI[where x=k])
-
-lemma set_cts_order_incl_kvs_tids:
-  assumes "CO_not_No_Ver gs k"
-  shows "set (cts_order gs k) \<subseteq> kvs_txids (kvs_of_s gs)"
-  using assms
-  by (auto simp add: kvs_txids_def dest: set_cts_order_incl_kvs_writers)
-
-
-
-(*****)
-
-
-
-(******************)
-(******************)
-(******************)
-
-
-subsubsection \<open>Write commit guard properties\<close>
-
-lemma write_commit_txn_to_vers_get_wtxn:
-  assumes "write_commit cl kv_map commit_t sn u'' clk mmap gs gs'" 
-  and "kv_map k = Some v" 
-  shows "txn_to_vers gs k (get_wtxn gs cl) = new_vers (Tn (Tn_cl sn cl)) v"
-  using assms
-  by (auto simp add: write_commit_def write_commit_G_def txn_to_vers_def
-      dest!: bspec[where x=k] split: ver_state.split)
-(*
-lemma write_commit_extended_view:    (* NOT USED? *)
-  assumes "write_commit cl kv_map commit_t sn u'' clk mmap gs gs'" 
-  shows "u'' = view_of (cts_order gs) (cl_ctx (cls gs cl))"
-  using assms
-  by (simp add: write_commit_def)
-
-lemma write_commit_seqn:    (* NOT USED? *)
-  assumes "write_commit cl kv_map commit_t sn u'' clk mmap gs gs'" 
-  shows "sn = cl_sn (cls gs cl)"
-  using assms
-  by (simp add: write_commit_def write_commit_G_def)
-
-lemmas write_commit_guard_simps = 
-  write_commit_txn_to_vers_get_wtxn write_commit_extended_view write_commit_seqn
-*)
-
-subsubsection \<open>Write commit update properties\<close>
-
-(*
-lemma write_commit_cl_sn_update:
-  assumes "write_commit cl kv_map commit_t sn u'' clk mmap gs gs'"
-  shows "cl_sn (cls gs' cl') = cl_sn (cls gs cl')"
-  using assms
-  by (auto simp add: write_commit_def) 
-*)
-
-lemma write_commit_txn_to_vers_pres:
-  assumes "write_commit_s cl kv_map cts sn u'' clk mmap gs gs'"
-  shows "txn_to_vers gs' k = txn_to_vers gs k"
-  using assms
-  by (auto 3 4 simp add: tps_trans_defs txn_to_vers_def split: ver_state.split)
-
-
-lemma write_commit_cts_order_update:
-  assumes "write_commit_s cl kv_map cts sn u'' clk mmap gs gs'"
-  shows "cts_order gs' k = 
-         (if kv_map k = None
-          then cts_order gs k
-          else insort_key (unique_ts ((wtxn_cts gs) (get_wtxn gs cl \<mapsto> cts))) (get_wtxn gs cl) (cts_order gs k))"
-  using assms
-  by (auto simp add: tps_trans_defs ext_corder_def)
-
-
-lemma write_commit_kvs_of_s:
-  assumes "write_commit_s cl kv_map cts sn u'' clk mmap s s'"
-  shows "kvs_of_s s' = update_kv (Tn_cl sn cl)
-                          (write_only_fp kv_map)
-                          (view_of (cts_order s) (get_view s cl))
-                          (kvs_of_s s)"
-  using assms
+  apply (auto simp add: get_view_def wtxns_dom_def)
   apply (intro ext)
-  apply (auto simp add: kvs_of_s_def update_kv_write_only write_commit_txn_to_vers_pres
-      write_commit_cts_order_update write_commit_txn_to_vers_get_wtxn split: option.split)
-  apply (simp add: tps_trans_defs) sorry
+  by auto
 
-(* the one above NEEDS THE WELL-ORDERED INVARIANT
-
-
-NO LONGER HOLDS
-lemma write_commit_views_of_s:
-  assumes "write_commit cl kv_map commit_t sn u'' clk mmap s s'"
-  shows "views_of_s s' = 
-         (\<lambda>cl'. view_of (ext_corder (get_wtxn s cl) kv_map (cts_order s))    
-                        (if cl' = cl then insert (get_wtxn s cl) (get_view s cl) 
-                         else get_view s cl'))"
-  using assms
-  by (auto simp add: write_commit_def write_commit_G_def write_commit_U_def views_of_s_def)
-*)
+lemma get_view_update_svr_commit:
+   "cl \<noteq> get_cl_w t \<Longrightarrow>
+    svr_state (svrs s k) t = Prep pd ts v \<Longrightarrow>
+    get_view (s\<lparr>svrs := (svrs s)
+                   (k := svrs s k
+                      \<lparr>svr_state := (svr_state (svrs s k))(t := Commit cts sts lst v rs),
+                       svr_clock := clk,
+                       svr_lst := sclk \<rparr>)\<rparr>) cl
+ = get_view s cl"
+  apply (auto simp add: get_view_def wtxns_dom_def)
+  apply (intro ext)
+  by auto
 
 
-lemmas write_commit_update_simps = 
-  write_commit_txn_to_vers_pres write_commit_cts_order_update write_commit_kvs_of_s
-  (*write_commit_views_of_s*)
+lemmas get_view_update_lemmas = 
+  get_view_update_cls get_view_update_cls_rtxn_rts get_view_update_cls_wtxn_cts_cts_order
+  get_view_update_svr_wtxns_dom get_view_update_svr_prep get_view_update_svr_commit
 
-(**************************************)
-
-
-lemma full_view_elem: "i \<in> full_view vl \<longleftrightarrow> i < length vl"
-  by (simp add: full_view_def)
-
-
-lemma length_update_kv_bound:
-  "i < length (update_kv t F u K k) \<longleftrightarrow> i < length (K k) \<or> W \<in> dom (F k) \<and> i = length (K k)"
-  by (smt (verit) Nat.not_less_eq domIff not_less_iff_gr_or_eq update_kv_length)
-
-(***************************************)
-
-
-lemma v_writer_set_cts_order_eq:
-  assumes "CO_not_No_Ver s k"                   
-  shows "v_writer ` set (kvs_of_s s k) = set (cts_order s k)"
-  using assms
-  apply (auto simp add:  CO_not_No_Ver_def kvs_of_s_defs image_def split: ver_state.split)
-   apply (metis (mono_tags, lifting) is_committed.cases version.select_convs(2))
-   subgoal for t apply (cases "svr_state (svrs s k) t", simp)
-      apply (metis (opaque_lifting) ver_state.distinct(5) ver_state.inject(1) version.select_convs(2))
-     subgoal for cts sts lst v rs apply (rule exI[where x="\<lparr>v_value = v, v_writer = t,
-          v_readerset = {t. \<exists>rts rlst. rs t = Some (rts, rlst) \<and> get_sn t < cl_sn (cls s (get_cl t))}\<rparr>"], simp)
-       by (rule bexI[where x=t], auto)
-     done
-   done
-
-subsubsection \<open>View Wellformedness\<close>
-
-definition FTid_notin_Get_View where
-  "FTid_notin_Get_View s cl \<longleftrightarrow> (\<forall>n cl' k. (n > cl_sn (cls s cl) \<longrightarrow> Tn (Tn_cl n cl) \<notin> get_view s cl' k) \<and>
-    (cl' \<noteq> cl \<longrightarrow> get_wtxn s cl \<notin> get_view s cl' k))"
-
-lemmas FTid_notin_Get_ViewI = FTid_notin_Get_View_def[THEN iffD2, rule_format]
-lemmas FTid_notin_Get_ViewE[elim] = FTid_notin_Get_View_def[THEN iffD1, elim_format, rule_format]
-
-lemma reach_ftid_notin_get_view [simp]: "reach tps_s s \<Longrightarrow> FTid_notin_Get_View s cl"
-proof(induction s rule: reach.induct)
-  case (reach_init s)
-  then show ?case by (auto simp add: FTid_notin_Get_View_def tps_s_defs get_view_def)
-next
-  case (reach_trans s e s')
-  then show ?case
-  proof (induction e)
-    case (RInvoke x1 x2 x3 x4)
-    then show ?case sorry
-  next
-    case (Read x1 x2 x3 x4 x5 x6 x7)
-    then show ?case sorry
-  next
-    case (RDone x1 x2 x3 x4 x5)
-    then show ?case sorry
-  next
-    case (WInvoke x1 x2 x3 x4)
-    then show ?case sorry
-  next
-    case (WCommit x1 x2 x3 x4 x5 x6 x7)
-    then show ?case sorry
-  next
-    case (WDone x1 x2 x3 x4 x5)
-    then show ?case sorry
-  next
-    case (RegR x1 x2 x3 x4 x5 x6 x7)
-    then show ?case sorry
-  next
-    case (PrepW x1 x2 x3 x4 x5)
-    then show ?case sorry
-  next
-    case (CommitW x1 x2 x3 x4 x5 x6 x7)
-    then show ?case sorry
-  qed
-qed
-
-lemma views_of_s_inv:
-  assumes "state_trans s e s'"
-    and "reach tps_s s"
-    and "\<not>commit_ev e"
-  shows "views_of_s s' cl = views_of_s s cl"
-  using assms using kvs_of_s_inv[of s e s']
-proof (induction e)
-  case (RInvoke x1 x2 x3 x4)
-  then show ?case apply (auto simp add: views_of_s_def tps_trans_defs get_view_def) sorry (* CHECK: does this even hold? *)
-next
-  case (RegR x1 x2 x3 x4 x5 x6 x7)
-  then show ?case apply (auto simp add: views_of_s_def tps_trans_defs get_view_def
-        add_to_readerset_def split: ver_state.split)
-    sorry
-next
-  case (PrepW x1 x2 x3 x4 x5)
-  then show ?case apply (auto simp add: views_of_s_def tps_trans_defs get_view_def) sorry
-next
-  case (CommitW x1 x2 x3 x4 x5 x6 x7)
-  then show ?case apply (auto simp add: views_of_s_def tps_trans_defs get_view_def) sorry
-qed (auto simp add: views_of_s_def tps_trans_defs get_view_def)
-
-lemma read_commit_views_of_s_other_cl_inv:
-  assumes "read_done cl kv_map sn u clk s s'"
-    and "reach tps_s s"
-    and "cl' \<noteq> cl"
-  shows "views_of_s s' cl' = views_of_s s cl'"
-  using assms
-  apply (auto simp add: tps_trans_defs views_of_s_def get_view_def) sorry
-
-lemma write_commit_views_of_s_other_cl_inv:
-  assumes "write_commit_s cl kv_map cts sn u'' clk mmap s s'"
-    and "reach tps_s s"
-    and "cl' \<noteq> cl"
-  shows "views_of_s s' cl' = views_of_s s cl'"
-proof -
-  have dist: "\<And>k. distinct (cts_order s' k)"
-    using assms CO_Distinct_def reach_co_distinct
-    by (metis state_trans.simps(5) tps_trans reach_trans)
-  have "\<And>k. (set (cts_order s' k) - set (cts_order s k)) \<inter> (get_view s cl' k) = {}"
-    using assms FTid_notin_Get_View_def[of s]
-    by (auto simp add: tps_trans_defs ext_corder_def set_insort_key)
-  then show ?thesis using assms dist view_of_prefix
-    apply (auto simp add: tps_trans_all_defs views_of_s_def get_view_def) sorry
-qed
-
-lemma reach_kvs_expands [simp]:
-  assumes "state_trans s e s'"
-    and "reach tps_s s"
-  shows "kvs_of_s s \<sqsubseteq>\<^sub>k\<^sub>v\<^sub>s kvs_of_s s'"
-  using assms kvs_of_s_inv[of s e s']
-proof (induction e)
-  case (RDone x1 x2 x3 x4 x5)
-  then show ?case
-    by (auto simp add: tps_trans_defs kvs_expands_def vlist_order_def version_order_def kvs_of_s_defs
-        view_atomic_def full_view_def split: ver_state.split)
-next
-  case (WCommit x1 x2 x3 x4 x5 x6 x7)
-  then show ?case using t_is_fresh[of s] write_commit_kvs_of_s[of _ x2]
-    apply (auto simp add: tps_trans_defs) by (meson kvs_expands_through_update)
-qed auto
-
-definition Views_of_s_Wellformed where
-  "Views_of_s_Wellformed s cl \<longleftrightarrow> (view_wellformed (kvs_of_s s) (views_of_s s cl))"
-
-lemmas Views_of_s_WellformedI = Views_of_s_Wellformed_def[THEN iffD2, rule_format]
-lemmas Views_of_s_WellformedE[elim] = Views_of_s_Wellformed_def[THEN iffD1, elim_format, rule_format]
-
-lemma reach_views_of_s_wellformed [simp]: "reach tps_s s \<Longrightarrow> Views_of_s_Wellformed s cl"
-proof(induction s rule: reach.induct)
-  case (reach_init s)
-  then show ?case
-    by (auto simp add: Views_of_s_Wellformed_def tps_s_defs view_of_def views_of_s_def the_T0
-        view_wellformed_defs full_view_def get_view_def kvs_of_s_defs)
-next
-  case (reach_trans s e s')
-  then show ?case using kvs_of_s_inv[of s e s'] reach_kvs_expands[of s e s']
-  proof (induction e)
-    case (RInvoke x1 x2 x3 x4)
-  then show ?case sorry
-next
-  case (RDone x1 x2 x3 x4 x5)
-    hence "view_wellformed (kvs_of_s s') (views_of_s s cl)" apply simp
-    using kvs_expanded_view_wellformed by blast
-    then show ?case using RDone
-    apply (auto simp add: Views_of_s_Wellformed_def) sorry
-  next
-    case (WCommit x1 x2 x3 x4 x5 x6 x7)
-    then show ?case
-      apply (simp add: Views_of_s_Wellformed_def tps_trans_defs views_of_s_def get_view_def) sorry
-  next
-    case (RegR x1 x2 x3 x4 x5 x6 x7)
-    then show ?case apply (auto simp add: Views_of_s_Wellformed_def tps_trans_defs
-          add_to_readerset_def split: ver_state.split) sorry
-  next
-    case (PrepW x1 x2 x3 x4 x5)    then show ?case apply (auto simp add: Views_of_s_Wellformed_def tps_trans_defs views_of_s_def get_view_def) sorry
-  next
-    case (CommitW x1 x2 x3 x4 x5 x6 x7)
-    then show ?case apply (auto simp add: Views_of_s_Wellformed_def tps_trans_defs views_of_s_def get_view_def) sorry
-  qed (auto simp add: Views_of_s_Wellformed_def tps_trans_defs views_of_s_def get_view_def)
-qed
-
-
-(**************************************)
-(**************************************)
-
-subsection \<open>Refinement Proof\<close>
-
-definition invariant_list where
-  "invariant_list s \<equiv> (\<forall>cl k. Sqn_Inv_c s cl \<and> Sqn_Inv_nc s cl
-    \<and> Views_of_s_Wellformed s cl \<and> Rtxn_Fp_Inv s cl \<and> CO_Distinct s k
-    \<and> T0_in_CO s k \<and> T0_First_in_CO s k \<and> View_Init s cl k \<and> FTid_notin_Get_View s cl)"
-
-lemma invariant_listE [elim]: 
-  "\<lbrakk> invariant_list s; 
-     \<lbrakk> \<And>cl. Sqn_Inv_c s cl; \<And>cl. Sqn_Inv_nc s cl;
-       \<And>cl. Rtxn_Fp_Inv s cl; \<And>k. CO_Distinct s k;
-       \<And>k. T0_in_CO s k; \<And>k. T0_First_in_CO s k; FTid_notin_Get_View s cl \<rbrakk>
-      \<Longrightarrow> P\<rbrakk> 
-   \<Longrightarrow> P"
-  by (auto simp add: invariant_list_def)
-
-lemma invariant_list_inv [simp, intro]:
-  "reach tps_s s \<Longrightarrow> invariant_list s"
-  by (auto simp add: invariant_list_def)     \<comment> \<open>should work with just "auto"?\<close>
-
-lemma tps_refines_et_es: "tps_s \<sqsubseteq>\<^sub>med ET_CC.ET_ES"
-proof (intro simulate_ES_fun)
-  fix gs0 :: "'v global_conf"
-  assume p: "init tps_s gs0"
-  then show "init ET_CC.ET_ES (sim gs0)"
-    by (auto simp add: ET_CC.ET_ES_defs tps_s_defs sim_defs kvs_init_def v_list_init_def 
-                       version_init_def get_view_def view_of_def the_T0)
-next
-  fix gs a and gs' :: "'v global_conf"
-  assume p: "tps_s: gs\<midarrow>a\<rightarrow> gs'" and reach_s: "reach tps_s gs" and "reach ET_CC.ET_ES (sim gs)"
-  then have I: "invariant_list gs" and reach_s': "reach tps_s gs'" by auto
-  show "ET_CC.ET_ES: sim gs\<midarrow>med a\<rightarrow> sim gs'"
-  using p I reach_s kvs_of_s_inv[of gs a gs'] views_of_s_inv[of gs a gs']
-  proof (induction a)
-    case (RDone cl kv_map sn u'' clk)
-    then show ?case
-    proof -
-      {
-        assume cmt: \<open>read_done_s cl kv_map sn u'' clk gs gs'\<close>
-        let ?u'' = "view_of (cts_order gs) (get_view gs cl)"
-        have \<open>ET_CC.ET_trans_and_fp 
-                (kvs_of_s gs, views_of_s gs)
-                 (ET cl sn u'' (read_only_fp kv_map))
-                (kvs_of_s gs', views_of_s gs')\<close>
-        proof (rule ET_CC.ET_trans_rule [where u'="views_of_s gs' cl"])
-          show \<open>views_of_s gs cl \<sqsubseteq> u''\<close> using cmt
-            by (auto simp add: read_done_s_def read_done_G_s_def read_done_U_def views_of_s_def
-                view_of_deps_mono)
-        next
-          show \<open>ET_CC.canCommit (kvs_of_s gs) u''
-                 (read_only_fp kv_map)\<close> using cmt I
-            sorry
-        next
-          show \<open>vShift_MR_RYW (kvs_of_s gs) u'' (kvs_of_s gs') (views_of_s gs' cl)\<close> using cmt I
-            apply (auto simp add: read_done_def vShift_MR_RYW_def vShift_MR_def vShift_RYW_def views_of_s_def)
-            \<comment> \<open>1. (writer_ver_i, t) \<in> SO \<Longrightarrow> t \<in> K'\K \<Longrightarrow> i \<in> view_of corder (cl_ctx \<union> get_ctx)
-                2. writer_ver_i \<in> K'\K \<Longrightarrow> i \<in> view_of corder (cl_ctx \<union> get_ctx)\<close> 
-            
-            
-            sorry
-        next
-          show \<open>view_wellformed (kvs_of_s gs) u''\<close> using cmt I
-            apply (auto simp add: read_done_s_def) sorry
-        next
-          show \<open>view_wellformed (kvs_of_s gs') (views_of_s gs' cl)\<close> using I
-            by (metis Views_of_s_Wellformed_def p reach_s reach_trans reach_views_of_s_wellformed)
-        next
-          show \<open>view_wellformed (kvs_of_s gs) (views_of_s gs cl)\<close> using cmt I
-            by (auto simp add: read_done_def read_done_G_def read_done_U_def invariant_list_def)
-        next
-          show \<open>Tn_cl sn cl \<in> next_txids (kvs_of_s gs) cl\<close> using cmt I
-            by (auto simp add: read_done_s_def read_done_G_s_def read_done_G_def t_is_fresh)
-        next
-          show \<open>fp_property (read_only_fp kv_map) (kvs_of_s gs) u''\<close>
-            using cmt I
-            by (auto simp add: read_done_s_def read_done_G_s_def read_done_G_def fp_property_def
-                  view_snapshot_def Rtxn_Fp_Inv_def read_only_fp_def invariant_list_def)
-        next
-          show \<open>kvs_of_s gs' = update_kv (Tn_cl sn cl)
-                (read_only_fp kv_map) u'' (kvs_of_s gs)\<close> using cmt I
-            apply (auto simp add: read_done_s_def) sorry
-        next
-          show \<open>views_of_s gs' = (views_of_s gs)(cl := views_of_s gs' cl)\<close> using cmt
-            by (auto simp add: read_done_s_def read_done_G_s_def read_done_G_def read_done_U_def
-                views_of_s_def get_view_def)
-        qed
-      }
-      then show ?thesis using RDone
-        by (auto simp only: ET_CC.trans_ET_ES_eq tps_trans state_trans.simps sim_def med.simps)
-    qed
-  next
-    case (WCommit cl kv_map cts sn u'' clk mmap)
-    then show ?case
-    proof -
-      {
-        assume cmt: \<open>write_commit_s cl kv_map cts sn u'' clk mmap gs gs'\<close>
-        have \<open>ET_CC.ET_trans_and_fp 
-                (kvs_of_s gs, views_of_s gs)
-                 (ET cl sn u'' (write_only_fp kv_map))
-                (kvs_of_s gs', views_of_s gs')\<close>
-        proof (rule ET_CC.ET_trans_rule [where u'="views_of_s gs' cl"])
-          show \<open>views_of_s gs cl \<sqsubseteq> u''\<close> using cmt
-            by (auto simp add: write_commit_s_def write_commit_G_s_def get_view_def 
-                views_of_s_def view_of_deps_mono)
-        next
-          show \<open>ET_CC.canCommit (kvs_of_s gs) u'' (write_only_fp kv_map)\<close> using cmt I
-            (*by (simp add: write_commit_def Deps_Closed_def closed_closed' ET_CC.canCommit_def
-                          invariant_list_def)*) sorry
-        next
-         show \<open>vShift_MR_RYW (kvs_of_s gs) u'' (kvs_of_s gs') (views_of_s gs' cl)\<close> 
-            using cmt I reach_s 
-            apply (intro vShift_MR_RYW_I)
-            subgoal  (* MR *)
-              using reach_s'[THEN reach_co_distinct] CO_Distinct_def
-              apply (auto simp add: write_commit_s_def write_commit_G_s_def write_commit_U_def) sorry
-                  (*views_of_s_cls_update intro: view_of_ext_corder_cl_ctx)*) (* Continue Here! *)
-
-            subgoal for t k i (* RYW.1: reflexive case *)
-              apply (auto 4 3 simp add: write_commit_update_simps kvs_txids_update_kv_write_only
-                                    length_update_kv_bound update_kv_v_writer_old full_view_elem
-                          dest: v_writer_in_kvs_txids
-                          split: if_split_asm)
-              (*by (auto simp add: ext_corder_def length_cts_order intro!: view_of_update
-                         dest!: reach_co_not_no_ver set_cts_order_incl_kvs_tids
-                         dest: write_commit_seqn v_writer_in_kvs_txids)*) sorry
-
-(**) 
-            thm write_commit_def
-
-            thm (*view_of_update*) view_of_mono (*views_of_s_cls_update*) length_cts_order
-
-            thm reach_co_not_no_ver set_cts_order_incl_kvs_tids
-
-(* all-in-one proof unfolding write_commit_def:
- 
-              apply (frule write_commit_kvs_of_s)
-              by (auto simp add: write_commit_def ext_corder_def views_of_s_cls_update v_writer_in_kvs_txids
-                                 update_kv_write_only length_update_kv nth_append length_cts_order
-                       intro!: view_of_update
-                       dest!: reach_co_not_no_ver set_cts_order_incl_kvs_tids
-                       split: option.split_asm if_split_asm)
-*)
-
-            subgoal for t k i  (* RYW.2: SO case *)
-              apply (auto simp add: write_commit_update_simps kvs_txids_update_kv_write_only
-                                    length_update_kv_bound update_kv_v_writer_old full_view_elem
-                          split: if_split_asm) sorry
-              (*subgoal for k' v' sorry
-
-                (* Do we need the closedness property here? *)
-                apply (clarsimp simp add: write_commit_def  )*)
-(*
-\<lbrakk> get_wtxn gs cl \<notin> kvs_txids (kvs_of_s gs); (v_writer (kvs_of_s gs k ! i), get_wtxn gs cl) \<in> SO; 
- i < length (kvs_of_s gs k); 
- sn = cl_sn (cls gs cl); 
- u'' = view_of (cts_order gs) (cl_ctx (cls gs cl));
- cl_state (cls gs cl) = WtxnPrep kv_map;
- \<forall>k\<in>dom kv_map. \<exists>pd ts v. svr_state (svrs gs k) (get_wtxn gs cl) = Prep pd ts v \<and> kv_map k = Some v;
- ....
-\<rbrakk>
-\<Longrightarrow> i \<in> view_of (ext_corder (get_wtxn gs cl) kv_map (cts_order gs)) (cl_ctx (cls gs cl) \<union> dom kv_map \<times> {get_wtxn gs cl}) k 
-*)
-
-                thm CO_is_Cmt_Abs_def    (* check this out *)
-
-
-                sorry
-              (*subgoal for k' v' v
-                by (metis SO_irreflexive update_kv_v_writer_new write_only_fp_write)
-              done
-            done*)
-        next
-          show \<open>view_wellformed (kvs_of_s gs) u''\<close> using cmt I
-            apply (auto simp add: write_commit_s_def write_commit_G_s_def view_wellformed_defs) 
-            subgoal using T0_First_in_CO_def[of gs] T0_in_CO_def[of gs] CO_Distinct_def[of gs] View_Init_def[of gs cl]
-              apply (auto simp add: view_of_def) apply (rule exI[where x=T0], auto) sorry
-            subgoal sorry
-            subgoal sorry
-            done
-        next
-          show \<open>view_wellformed (kvs_of_s gs') (views_of_s gs' cl)\<close>
-            by (metis (no_types, lifting) Views_of_s_Wellformed_def p reach_s reach_trans
-                      reach_views_of_s_wellformed)
-        next
-          show \<open>view_wellformed (kvs_of_s gs) (views_of_s gs cl)\<close> using cmt I
-            by (auto simp add: write_commit_s_def write_commit_G_s_def write_commit_G_def
-                write_commit_U_def invariant_list_def)
-        next
-          show \<open>Tn_cl sn cl \<in> next_txids (kvs_of_s gs) cl\<close> using cmt I
-            by (auto simp add: write_commit_s_def write_commit_G_s_def write_commit_G_def t_is_fresh)
-        next
-          show \<open>fp_property (write_only_fp kv_map) (kvs_of_s gs) u''\<close>
-            by (simp add: fp_property_write_only_fp)
-        next
-          show \<open>kvs_of_s gs' = update_kv (Tn_cl sn cl) (write_only_fp kv_map) u'' (kvs_of_s gs)\<close> 
-            using cmt apply (simp add: write_commit_s_def write_commit_G_s_def)
-            by (metis cmt write_commit_kvs_of_s)
-        next
-          show \<open>views_of_s gs' = (views_of_s gs)(cl := views_of_s gs' cl)\<close> using cmt
-            apply (auto simp add: write_commit_s_def) apply (rule ext)
-            by (smt (verit) cmt fun_upd_apply reach_ftid_notin_get_view reach_co_distinct reach_s reach_s'
-                write_commit_views_of_s_other_cl_inv)
-        qed
-      }
-      then show ?thesis using WCommit
-        by (auto simp only: ET_CC.trans_ET_ES_eq tps_trans state_trans.simps sim_def med.simps)
-    qed
-  qed (auto simp add: sim_def views_of_s_def get_view_def tps_trans_defs invariant_list_def)
-qed
 
 end
