txn-data-consistency/EP+_Sorted_eq_E.thy
@@ -6,29 +6,6 @@ begin
 
 subsubsection \<open>Lemmas\<close>
 
-lemma init_tps_tps_s_eq:
-  "init tps_s s \<longleftrightarrow> init tps s"
-  by (simp add: tps_def tps_s_defs)
-
-lemma tps_s_ev_sub_tps:
-  "tps_s: s\<midarrow>e\<rightarrow> s' \<Longrightarrow> tps: s\<midarrow>e\<rightarrow> s'"
-  by (induction e) (auto simp add: read_done_s_def read_done_def read_done_G_s_def
-      write_commit_s_def write_commit_def write_commit_G_s_def)
-
-lemma tps_s_tr_sub_tps:
-  "(tps_s: s \<midarrow>\<langle>\<tau>\<rangle>\<rightarrow> s') \<Longrightarrow> (tps: s \<midarrow>\<langle>\<tau>\<rangle>\<rightarrow> s')"
-  apply (induction \<tau> s' rule: trace.induct, auto)
-  by (metis tps_trans tps_s_ev_sub_tps trace_snoc)
-
-lemma reach_tps: "reach tps_s s \<Longrightarrow> reach tps s" \<comment> \<open>All tps invs can also be used for tps_s\<close>
-proof (induction s rule: reach.induct)
-  case (reach_init s)
-  then show ?case by (simp add: init_tps_tps_s_eq)
-next
-  case (reach_trans s e s')
-  then show ?case using tps_s_ev_sub_tps[of s e s'] by auto
-qed
-
 \<comment> \<open>tps_s \<longrightarrow> good execs\<close> 
 
 lemma reach_good_state_f_None:
